<?xml version="1.0" encoding="UTF-8"?>
<rdf:RDF xmlns:rdf="http://www.w3.org/1999/02/22-rdf-syntax-ns#" xmlns:schema="http://schema.org/" xmlns:col="http://os.uk/vocabularies/collection/" xmlns:owl="http://www.w3.org/2002/07/owl#" xmlns:org="http://www.w3.org/ns/org#" xmlns:xsd="http://www.w3.org/2001/XMLSchema#" xmlns:skosthes="http://purl.org/iso25964/skos-thes#" xmlns:rdfs="http://www.w3.org/2000/01/rdf-schema#" xmlns:ngd="http://os.uk/vocabularies/ngd/#" xmlns:qb="http://purl.org/linked-data/cube#" xmlns:dct="http://purl.org/dc/terms/" xmlns:sh="http://www.w3.org/ns/shacl#" xmlns:topic="https://inspire.ec.europa.eu/metadata-codelist/TopicCategory/" xmlns:theme="http://os.uk/vocabularies/theme/" xmlns:insp-theme="https://inspire.ec.europa.eu/theme/" xmlns:dcat="http://www.w3.org/ns/dcat#" xmlns:prov="http://www.w3.org/ns/prov#" xmlns:foaf="http://xmlns.com/foaf/0.1/" xmlns:dc="http://purl.org/dc/elements/1.1/" xmlns:skos="http://www.w3.org/2004/02/skos/core#" xmlns:skosxl="http://www.w3.org/2008/05/skos-xl#" xmlns:euvoc="http://publications.europa.eu/ontology/euvoc#">
  <rdf:Description rdf:about="http://os.uk/vocabularies/ngd">
    <rdf:type rdf:resource="http://www.w3.org/2004/02/skos/core#ConceptScheme" />
    <dct:title xml:lang="en">Ordnance Survey NGD vocabulary</dct:title>
    <dct:description xml:lang="en">Pre-release trial SKOS version of evolving NGD vocab, 2022-02-15 extract from NGD_Metadata_And_Definitions_MASTER</dct:description>
  </rdf:Description>
  <rdf:Description rdf:about="http://os.uk/vocabularies/ngd/BoundaryHighWaterMark">
    <rdf:type rdf:resource="http://www.w3.org/2004/02/skos/core#Concept" />
    <skos:prefLabel xml:lang="en">Boundary High Water Mark</skos:prefLabel>
    <skos:definition xml:lang="en">The alignment of the Mean High Water mark in England &amp; Wales or the Mean High Water Springs mark in Scotland, at a level of detail consistent with the boundary polygons. In places where there are vertical cliffs and walls, the line is coincident with the boundary polygon perimeter, otherwise it will be inside, enclosing the intertidal area.</skos:definition>
    <skos:altLabel xml:lang="en">Boundary High Water Mark</skos:altLabel>
    <skos:broader rdf:resource="http://os.uk/vocabularies/collection/Boundaries" />
    <skos:broader rdf:resource="https://inspire.ec.europa.eu/metadata-codelist/TopicCategory/boundaries" />
    <skos:broader rdf:resource="https://inspire.ec.europa.eu/theme/au" />
    <skos:broader rdf:resource="http://inspire.ec.europa.eu/featureconcept/AdministrativeBoundary" />
    <skos:inScheme rdf:resource="http://os.uk/vocabularies/ngd" />
  </rdf:Description>
  <rdf:Description rdf:about="http://os.uk/vocabularies/ngd/BuildingLine">
    <rdf:type rdf:resource="http://www.w3.org/2004/02/skos/core#Concept" />
    <skos:prefLabel xml:lang="en">Building Line</skos:prefLabel>
    <skos:definition xml:lang="en">Either a wall between two buildings or the external alignment of an overhead building or canopy.</skos:definition>
    <skos:altLabel xml:lang="en">Building Line</skos:altLabel>
    <skos:broader rdf:resource="http://os.uk/vocabularies/collection/Building-Features" />
    <skos:broader rdf:resource="https://inspire.ec.europa.eu/metadata-codelist/TopicCategory/structure" />
    <skos:broader rdf:resource="https://inspire.ec.europa.eu/theme/bu" />
    <skos:broader rdf:resource="http://inspire.ec.europa.eu/featureconcept/Building" />
    <skos:inScheme rdf:resource="http://os.uk/vocabularies/ngd" />
  </rdf:Description>
  <rdf:Description rdf:about="http://os.uk/vocabularies/ngd/BuildingPart">
    <rdf:type rdf:resource="http://www.w3.org/2004/02/skos/core#Concept" />
    <skos:prefLabel xml:lang="en">Building Part</skos:prefLabel>
    <skos:definition xml:lang="en">Either a complete roofed structure or part of a larger roofed structure where internal divisions exist from ground to roof level and they can be identified externally.</skos:definition>
    <skos:altLabel xml:lang="en">Building Part</skos:altLabel>
    <skos:broader rdf:resource="http://os.uk/vocabularies/collection/Building-Features" />
    <skos:broader rdf:resource="https://inspire.ec.europa.eu/metadata-codelist/TopicCategory/structure" />
    <skos:broader rdf:resource="https://inspire.ec.europa.eu/theme/bu" />
    <skos:broader rdf:resource="http://inspire.ec.europa.eu/featureconcept/BuildingPart" />
    <skos:inScheme rdf:resource="http://os.uk/vocabularies/ngd" />
  </rdf:Description>
  <rdf:Description rdf:about="http://os.uk/vocabularies/ngd/BuiltAddress">
    <rdf:type rdf:resource="http://www.w3.org/2004/02/skos/core#Concept" />
    <skos:prefLabel xml:lang="en">Built Address</skos:prefLabel>
    <skos:definition xml:lang="en">An active address for a building or similar construction that can conceivably receive mail, deliveries or services.</skos:definition>
    <skos:altLabel xml:lang="en">Built Address</skos:altLabel>
    <skos:broader rdf:resource="http://os.uk/vocabularies/collection/GB-Address" />
    <skos:broader rdf:resource="http://os.uk/vocabularies/collection/Islands-Address" />
    <skos:broader rdf:resource="https://inspire.ec.europa.eu/metadata-codelist/TopicCategory/location" />
    <skos:broader rdf:resource="https://inspire.ec.europa.eu/theme/ad" />
    <skos:broader rdf:resource="http://inspire.ec.europa.eu/featureconcept/Address" />
    <skos:inScheme rdf:resource="http://os.uk/vocabularies/ngd" />
  </rdf:Description>
  <rdf:Description rdf:about="http://os.uk/vocabularies/ngd/CartographicRailDetail">
    <rdf:type rdf:resource="http://www.w3.org/2004/02/skos/core#Concept" />
    <skos:prefLabel xml:lang="en">Cartographic Rail Detail</skos:prefLabel>
    <skos:definition xml:lang="en">A continuous line of steel bars that as a set of parallel features guide the movement of a rail vehicle wheels.</skos:definition>
    <skos:altLabel xml:lang="en">Cartographic Rail Detail</skos:altLabel>
    <skos:broader rdf:resource="http://os.uk/vocabularies/collection/Transport-Features" />
    <skos:broader rdf:resource="https://inspire.ec.europa.eu/metadata-codelist/TopicCategory/transportation" />
    <skos:broader rdf:resource="https://inspire.ec.europa.eu/theme/tn" />
    <skos:inScheme rdf:resource="http://os.uk/vocabularies/ngd" />
  </rdf:Description>
  <rdf:Description rdf:about="http://os.uk/vocabularies/ngd/CartographicRoadTrackOrPathLine">
    <rdf:type rdf:resource="http://www.w3.org/2004/02/skos/core#Concept" />
    <skos:prefLabel xml:lang="en">Cartographic Road Track Or Path Line</skos:prefLabel>
    <skos:definition xml:lang="en">A manmade linear feature associated with associated with the passage of vehicles, pedestrians and animals being ridden or led not wide enough to capture as a RoadTrackOrPath.</skos:definition>
    <skos:altLabel xml:lang="en">Cartographic Road Track or Path Line</skos:altLabel>
    <skos:broader rdf:resource="http://os.uk/vocabularies/collection/Transport-Features" />
    <skos:broader rdf:resource="https://inspire.ec.europa.eu/metadata-codelist/TopicCategory/transportation" />
    <skos:broader rdf:resource="https://inspire.ec.europa.eu/theme/tn" />
    <skos:broader rdf:resource="http://inspire.ec.europa.eu/featureconcept/Road" />
    <skos:inScheme rdf:resource="http://os.uk/vocabularies/ngd" />
  </rdf:Description>
  <rdf:Description rdf:about="http://os.uk/vocabularies/ngd/CeremonialCounty">
    <rdf:type rdf:resource="http://www.w3.org/2004/02/skos/core#Concept" />
    <skos:prefLabel xml:lang="en">Ceremonial County</skos:prefLabel>
    <skos:definition xml:lang="en">An area that has a representative appointed by the monarch as a personal representative (Lord Lieutenant) or has a High Sheriff.</skos:definition>
    <skos:altLabel xml:lang="en">Ceremonial County</skos:altLabel>
    <skos:broader rdf:resource="http://os.uk/vocabularies/collection/Boundaries" />
    <skos:broader rdf:resource="https://inspire.ec.europa.eu/metadata-codelist/TopicCategory/boundaries" />
    <skos:broader rdf:resource="https://inspire.ec.europa.eu/theme/au" />
    <skos:broader rdf:resource="http://inspire.ec.europa.eu/featureconcept/AdministrativeUnit" />
    <skos:inScheme rdf:resource="http://os.uk/vocabularies/ngd" />
  </rdf:Description>
  <rdf:Description rdf:about="http://os.uk/vocabularies/ngd/CompoundStructure">
    <rdf:type rdf:resource="http://www.w3.org/2004/02/skos/core#Concept" />
    <skos:prefLabel xml:lang="en">Compound Structure</skos:prefLabel>
    <skos:definition xml:lang="en">A manmade construction built for a specific purpose.</skos:definition>
    <skos:altLabel xml:lang="en">Compound Structure</skos:altLabel>
    <skos:broader rdf:resource="http://os.uk/vocabularies/collection/Structure-Features" />
    <skos:broader rdf:resource="https://inspire.ec.europa.eu/metadata-codelist/TopicCategory/structure" />
    <skos:broader rdf:resource="https://inspire.ec.europa.eu/theme/bu" />
    <skos:inScheme rdf:resource="http://os.uk/vocabularies/ngd" />
  </rdf:Description>
  <rdf:Description rdf:about="http://os.uk/vocabularies/ngd/ConnectingLink">
    <rdf:type rdf:resource="http://www.w3.org/2004/02/skos/core#Concept" />
    <skos:prefLabel xml:lang="en">Connecting Link</skos:prefLabel>
    <skos:definition xml:lang="en">An indicative connection between the Path network and the Road network that may not reflect any specific real world feature or alignment.</skos:definition>
    <skos:altLabel xml:lang="en">Connecting Link</skos:altLabel>
    <skos:broader rdf:resource="http://os.uk/vocabularies/collection/Transport-Network" />
    <skos:broader rdf:resource="https://inspire.ec.europa.eu/metadata-codelist/TopicCategory/transportation" />
    <skos:broader rdf:resource="https://inspire.ec.europa.eu/theme/tn" />
    <skos:broader rdf:resource="http://inspire.ec.europa.eu/featureconcept/RoadLink" />
    <skos:inScheme rdf:resource="http://os.uk/vocabularies/ngd" />
  </rdf:Description>
  <rdf:Description rdf:about="http://os.uk/vocabularies/ngd/ConnectingNode">
    <rdf:type rdf:resource="http://www.w3.org/2004/02/skos/core#Concept" />
    <skos:prefLabel xml:lang="en">Connecting Node</skos:prefLabel>
    <skos:definition xml:lang="en">The location on the road network that indicates a connection to the Path Network.</skos:definition>
    <skos:altLabel xml:lang="en">Connecting Node</skos:altLabel>
    <skos:broader rdf:resource="http://os.uk/vocabularies/collection/Transport-Network" />
    <skos:broader rdf:resource="https://inspire.ec.europa.eu/metadata-codelist/TopicCategory/transportation" />
    <skos:broader rdf:resource="https://inspire.ec.europa.eu/theme/tn" />
    <skos:broader rdf:resource="http://inspire.ec.europa.eu/featureconcept/RoadNode" />
    <skos:inScheme rdf:resource="http://os.uk/vocabularies/ngd" />
  </rdf:Description>
  <rdf:Description rdf:about="http://os.uk/vocabularies/ngd/Country">
    <rdf:type rdf:resource="http://www.w3.org/2004/02/skos/core#Concept" />
    <skos:prefLabel xml:lang="en">Country</skos:prefLabel>
    <skos:definition xml:lang="en">A country is a distinct territorial body or political entity (i.e. a nation). Currenly includes England, Wales and Scotland.</skos:definition>
    <skos:broader rdf:resource="http://os.uk/vocabularies/collection/Boundaries" />
    <skos:broader rdf:resource="https://inspire.ec.europa.eu/metadata-codelist/TopicCategory/boundaries" />
    <skos:broader rdf:resource="https://inspire.ec.europa.eu/theme/au" />
    <skos:broader rdf:resource="http://inspire.ec.europa.eu/featureconcept/AdministrativeUnit" />
    <skos:inScheme rdf:resource="http://os.uk/vocabularies/ngd" />
  </rdf:Description>
  <rdf:Description rdf:about="http://os.uk/vocabularies/ngd/DevolvedParliamentConstituency">
    <rdf:type rdf:resource="http://www.w3.org/2004/02/skos/core#Concept" />
    <skos:prefLabel xml:lang="en">Devolved Parliament Constituency</skos:prefLabel>
    <skos:definition xml:lang="en">A parliamentary constituency in Scotland or Wales but not in England.</skos:definition>
    <skos:altLabel xml:lang="en">Devolved Parliament Constituency</skos:altLabel>
    <skos:broader rdf:resource="http://os.uk/vocabularies/collection/Boundaries" />
    <skos:broader rdf:resource="https://inspire.ec.europa.eu/metadata-codelist/TopicCategory/boundaries" />
    <skos:broader rdf:resource="https://inspire.ec.europa.eu/theme/au" />
    <skos:broader rdf:resource="http://inspire.ec.europa.eu/featureconcept/AdministrativeUnit" />
    <skos:inScheme rdf:resource="http://os.uk/vocabularies/ngd" />
  </rdf:Description>
  <rdf:Description rdf:about="http://os.uk/vocabularies/ngd/DevolvedParliamentElectoralRegion">
    <rdf:type rdf:resource="http://www.w3.org/2004/02/skos/core#Concept" />
    <skos:prefLabel xml:lang="en">Devolved Parliament Electoral Region</skos:prefLabel>
    <skos:definition xml:lang="en">An electoral region in Scotland or Wales but not in England.</skos:definition>
    <skos:altLabel xml:lang="en">Devolved Parliament Electoral Region</skos:altLabel>
    <skos:broader rdf:resource="http://os.uk/vocabularies/collection/Boundaries" />
    <skos:broader rdf:resource="https://inspire.ec.europa.eu/metadata-codelist/TopicCategory/boundaries" />
    <skos:broader rdf:resource="https://inspire.ec.europa.eu/theme/au" />
    <skos:broader rdf:resource="http://inspire.ec.europa.eu/featureconcept/AdministrativeUnit" />
    <skos:inScheme rdf:resource="http://os.uk/vocabularies/ngd" />
  </rdf:Description>
  <rdf:Description rdf:about="http://os.uk/vocabularies/ngd/ElectoralDivision">
    <rdf:type rdf:resource="http://www.w3.org/2004/02/skos/core#Concept" />
    <skos:prefLabel xml:lang="en">Electoral Division</skos:prefLabel>
    <skos:definition xml:lang="en">Electoral wards/divisions are the key building blocks of UK administrative geography. They are the spatial units used to elect local government councilors in metropolitan and non-metropolitan districts, unitary authorities and the London boroughs in England; unitary authorities in Wales and council areas in Scotland. Electoral divisions are specifically used in non-metropolitan counties, Welsh unitary authorities and some English unitary authorities.</skos:definition>
    <skos:altLabel xml:lang="en">Electoral Division</skos:altLabel>
    <skos:broader rdf:resource="http://os.uk/vocabularies/collection/Boundaries" />
    <skos:broader rdf:resource="https://inspire.ec.europa.eu/metadata-codelist/TopicCategory/boundaries" />
    <skos:broader rdf:resource="https://inspire.ec.europa.eu/theme/au" />
    <skos:broader rdf:resource="http://inspire.ec.europa.eu/featureconcept/AdministrativeUnit" />
    <skos:inScheme rdf:resource="http://os.uk/vocabularies/ngd" />
  </rdf:Description>
  <rdf:Description rdf:about="http://os.uk/vocabularies/ngd/FerryLink">
    <rdf:type rdf:resource="http://www.w3.org/2004/02/skos/core#Concept" />
    <skos:prefLabel xml:lang="en">Ferry Link</skos:prefLabel>
    <skos:definition xml:lang="en">A scheduled service between two ferry terminals for vehicles and or pedestrians.</skos:definition>
    <skos:altLabel xml:lang="en">Ferry Link</skos:altLabel>
    <skos:broader rdf:resource="http://os.uk/vocabularies/collection/Transport-Network" />
    <skos:broader rdf:resource="https://inspire.ec.europa.eu/metadata-codelist/TopicCategory/transportation" />
    <skos:broader rdf:resource="https://inspire.ec.europa.eu/theme/tn" />
    <skos:exactMatch rdf:resource="http://inspire.ec.europa.eu/featureconcept/FerryCrossing" />
    <skos:inScheme rdf:resource="http://os.uk/vocabularies/ngd" />
  </rdf:Description>
  <rdf:Description rdf:about="http://os.uk/vocabularies/ngd/FerryNode">
    <rdf:type rdf:resource="http://www.w3.org/2004/02/skos/core#Concept" />
    <skos:prefLabel xml:lang="en">Ferry Node</skos:prefLabel>
    <skos:definition xml:lang="en">The location at the end of the Ferry network where the user transitions to road or path.</skos:definition>
    <skos:altLabel xml:lang="en">Ferry Node</skos:altLabel>
    <skos:broader rdf:resource="http://os.uk/vocabularies/collection/Transport-Network" />
    <skos:broader rdf:resource="https://inspire.ec.europa.eu/metadata-codelist/TopicCategory/transportation" />
    <skos:broader rdf:resource="https://inspire.ec.europa.eu/theme/tn" />
    <skos:broader rdf:resource="http://inspire.ec.europa.eu/featureconcept/PortNode" />
    <skos:inScheme rdf:resource="http://os.uk/vocabularies/ngd" />
  </rdf:Description>
  <rdf:Description rdf:about="http://os.uk/vocabularies/ngd/FerryTerminal">
    <rdf:type rdf:resource="http://www.w3.org/2004/02/skos/core#Concept" />
    <skos:prefLabel xml:lang="en">Ferry Terminal</skos:prefLabel>
    <skos:definition xml:lang="en">An indicative connection between the Ferry Network and the Path or Road network.</skos:definition>
    <skos:altLabel xml:lang="en">Ferry Terminal</skos:altLabel>
    <skos:broader rdf:resource="http://os.uk/vocabularies/collection/Transport-Network" />
    <skos:broader rdf:resource="https://inspire.ec.europa.eu/metadata-codelist/TopicCategory/transportation" />
    <skos:broader rdf:resource="https://inspire.ec.europa.eu/theme/tn" />
    <skos:broader rdf:resource="http://inspire.ec.europa.eu/featureconcept/PortNode" />
    <skos:inScheme rdf:resource="http://os.uk/vocabularies/ngd" />
  </rdf:Description>
  <rdf:Description rdf:about="http://os.uk/vocabularies/ngd/GLAAssemblyConstituency">
    <rdf:type rdf:resource="http://www.w3.org/2004/02/skos/core#Concept" />
    <skos:prefLabel xml:lang="en">GLA Assembly Constituency</skos:prefLabel>
    <skos:definition xml:lang="en">Greater London Authority (GLA) Assembly constituencies are used to elect members to the London Assembly, which is part of the GLA.</skos:definition>
    <skos:altLabel xml:lang="en">Greater London Authority Assembly Constituency</skos:altLabel>
    <skos:broader rdf:resource="http://os.uk/vocabularies/collection/Boundaries" />
    <skos:broader rdf:resource="https://inspire.ec.europa.eu/metadata-codelist/TopicCategory/boundaries" />
    <skos:broader rdf:resource="https://inspire.ec.europa.eu/theme/au" />
    <skos:broader rdf:resource="http://inspire.ec.europa.eu/featureconcept/AdministrativeUnit" />
    <skos:inScheme rdf:resource="http://os.uk/vocabularies/ngd" />
  </rdf:Description>
  <rdf:Description rdf:about="http://os.uk/vocabularies/ngd/HighwayDedication">
    <rdf:type rdf:resource="http://www.w3.org/2004/02/skos/core#Concept" />
    <skos:prefLabel xml:lang="en">Highway Dedication</skos:prefLabel>
    <skos:definition xml:lang="en">Definition of which type of Highway user has access to a particular section of the Highway.</skos:definition>
    <skos:altLabel xml:lang="en">Highway Dedication</skos:altLabel>
    <skos:broader rdf:resource="http://os.uk/vocabularies/collection/RAMI" />
    <skos:broader rdf:resource="https://inspire.ec.europa.eu/metadata-codelist/TopicCategory/transportation" />
    <skos:broader rdf:resource="https://inspire.ec.europa.eu/theme/tn" />
    <skos:broader rdf:resource="http://inspire.ec.europa.eu/featureconcept/RestrictionForVehicles" />
    <skos:inScheme rdf:resource="http://os.uk/vocabularies/ngd" />
  </rdf:Description>
  <rdf:Description rdf:about="http://os.uk/vocabularies/ngd/HistoricAddress">
    <rdf:type rdf:resource="http://www.w3.org/2004/02/skos/core#Concept" />
    <skos:prefLabel xml:lang="en">Historic Address</skos:prefLabel>
    <skos:definition xml:lang="en">A former address for a building or similar construction that could conceivably receive mail, deliveries or services prior to becoming historic.</skos:definition>
    <skos:altLabel xml:lang="en">Historic Address</skos:altLabel>
    <skos:broader rdf:resource="http://os.uk/vocabularies/collection/GB-Address" />
    <skos:broader rdf:resource="http://os.uk/vocabularies/collection/Islands-Address" />
    <skos:broader rdf:resource="https://inspire.ec.europa.eu/metadata-codelist/TopicCategory/location" />
    <skos:broader rdf:resource="https://inspire.ec.europa.eu/theme/ad" />
    <skos:broader rdf:resource="http://inspire.ec.europa.eu/featureconcept/Address" />
    <skos:inScheme rdf:resource="http://os.uk/vocabularies/ngd" />
  </rdf:Description>
  <rdf:Description rdf:about="http://os.uk/vocabularies/ngd/HistoricCounty">
    <rdf:type rdf:resource="http://www.w3.org/2004/02/skos/core#Concept" />
    <skos:prefLabel xml:lang="en">Historic County</skos:prefLabel>
    <skos:definition xml:lang="en">Counties based on historic records and mapping circa 1888 and using the primary sources of the Local Government (England and Wales) Act 1888, the Local Government (Scotland) Act 1889 and the Sheriffs Act 1887. The historic counties dataset shows the county boundaries in place in 1888 in England and Wales and those established a year later in Scotland. The alignments of the counties for England and Wales are derived from mapping sourced from the National Archives and dating from 1890. The most recent available mapping dates for Scotland are from 1940.</skos:definition>
    <skos:altLabel xml:lang="en">Historic County</skos:altLabel>
    <skos:broader rdf:resource="http://os.uk/vocabularies/collection/Boundaries" />
    <skos:broader rdf:resource="https://inspire.ec.europa.eu/metadata-codelist/TopicCategory/boundaries" />
    <skos:broader rdf:resource="https://inspire.ec.europa.eu/theme/au" />
    <skos:broader rdf:resource="http://inspire.ec.europa.eu/featureconcept/AdministrativeUnit" />
    <skos:inScheme rdf:resource="http://os.uk/vocabularies/ngd" />
  </rdf:Description>
  <rdf:Description rdf:about="http://os.uk/vocabularies/ngd/HistoricEuropeanRegion">
    <rdf:type rdf:resource="http://www.w3.org/2004/02/skos/core#Concept" />
    <skos:prefLabel xml:lang="en">Historic European Region</skos:prefLabel>
    <skos:definition xml:lang="en">The electoral regions used for elections to the European Parliament when the UK was a member of the European Union.</skos:definition>
    <skos:altLabel xml:lang="en">Historic European Region</skos:altLabel>
    <skos:broader rdf:resource="http://os.uk/vocabularies/collection/Boundaries" />
    <skos:broader rdf:resource="https://inspire.ec.europa.eu/metadata-codelist/TopicCategory/boundaries" />
    <skos:broader rdf:resource="https://inspire.ec.europa.eu/theme/au" />
    <skos:broader rdf:resource="http://inspire.ec.europa.eu/featureconcept/AdministrativeUnit" />
    <skos:inScheme rdf:resource="http://os.uk/vocabularies/ngd" />
  </rdf:Description>
  <rdf:Description rdf:about="http://os.uk/vocabularies/ngd/InterTidalLine">
    <rdf:type rdf:resource="http://www.w3.org/2004/02/skos/core#Concept" />
    <skos:prefLabel xml:lang="en">Inter Tidal Line</skos:prefLabel>
    <skos:definition xml:lang="en">A watercourse extending across the intertidal zone.</skos:definition>
    <skos:altLabel xml:lang="en">Inter Tidal Line</skos:altLabel>
    <skos:broader rdf:resource="http://os.uk/vocabularies/collection/Water-Features" />
    <skos:broader rdf:resource="https://inspire.ec.europa.eu/metadata-codelist/TopicCategory/inlandWaters" />
    <skos:broader rdf:resource="https://inspire.ec.europa.eu/theme/hy" />
    <skos:broader rdf:resource="https://inspire.ec.europa.eu/featureconcept/Watercourse" />
    <skos:inScheme rdf:resource="http://os.uk/vocabularies/ngd" />
  </rdf:Description>
  <rdf:Description rdf:about="http://os.uk/vocabularies/ngd/Land">
    <rdf:type rdf:resource="http://www.w3.org/2004/02/skos/core#Concept" />
    <skos:prefLabel xml:lang="en">Land</skos:prefLabel>
    <skos:definition xml:lang="en">An area on the earth's surface that has not otherwise been captured as either a BuildingPart, Rail, RoadTrackOrPath, Structure or Water feature.</skos:definition>
    <skos:broader rdf:resource="http://os.uk/vocabularies/collection/Land-Features" />
    <skos:broader rdf:resource="https://inspire.ec.europa.eu/metadata-codelist/TopicCategory/imageryBaseMapsEarthCover" />
    <skos:broader rdf:resource="https://inspire.ec.europa.eu/theme/lc" />
    <skos:broader rdf:resource="http://inspire.ec.europa.eu/featureconcept/LandCoverUnit" />
    <skos:inScheme rdf:resource="http://os.uk/vocabularies/ngd" />
  </rdf:Description>
  <rdf:Description rdf:about="http://os.uk/vocabularies/ngd/Landform">
    <rdf:type rdf:resource="http://www.w3.org/2004/02/skos/core#Concept" />
    <skos:prefLabel xml:lang="en">Landform</skos:prefLabel>
    <skos:definition xml:lang="en">An area of the earth's surface with a distinct physical morphology such as cliffs, artificial slopes, ravines and some former mineral workings.</skos:definition>
    <skos:broader rdf:resource="http://os.uk/vocabularies/collection/Land-Features" />
    <skos:broader rdf:resource="https://inspire.ec.europa.eu/metadata-codelist/TopicCategory/environment" />
    <skos:inScheme rdf:resource="http://os.uk/vocabularies/ngd" />
  </rdf:Description>
  <rdf:Description rdf:about="http://os.uk/vocabularies/ngd/LandformLine">
    <rdf:type rdf:resource="http://www.w3.org/2004/02/skos/core#Concept" />
    <skos:prefLabel xml:lang="en">Landform Line</skos:prefLabel>
    <skos:definition xml:lang="en">The alignment of either the higher limit or the side or lower limit of areas with a distinct physical morphology, typically where there is a signficant change in slope angle.</skos:definition>
    <skos:altLabel xml:lang="en">Landform Line</skos:altLabel>
    <skos:broader rdf:resource="http://os.uk/vocabularies/collection/Land-Features" />
    <skos:broader rdf:resource="https://inspire.ec.europa.eu/metadata-codelist/TopicCategory/environment" />
    <skos:inScheme rdf:resource="http://os.uk/vocabularies/ngd" />
  </rdf:Description>
  <rdf:Description rdf:about="http://os.uk/vocabularies/ngd/LandformPoint">
    <rdf:type rdf:resource="http://www.w3.org/2004/02/skos/core#Concept" />
    <skos:prefLabel xml:lang="en">Landform Point</skos:prefLabel>
    <skos:definition xml:lang="en">An area of the earth's surface with a distinct physical morphology that is too small to capture as a Landform feature but that is considered to be of sufficient interest to be captured, typically associated with former mineral workings.</skos:definition>
    <skos:altLabel xml:lang="en">Landform Point</skos:altLabel>
    <skos:broader rdf:resource="http://os.uk/vocabularies/collection/Land-Features" />
    <skos:broader rdf:resource="https://inspire.ec.europa.eu/metadata-codelist/TopicCategory/environment" />
    <skos:inScheme rdf:resource="http://os.uk/vocabularies/ngd" />
  </rdf:Description>
  <rdf:Description rdf:about="http://os.uk/vocabularies/ngd/LowerTierLocalAuthority">
    <rdf:type rdf:resource="http://www.w3.org/2004/02/skos/core#Concept" />
    <skos:prefLabel xml:lang="en">Lower Tier Local Authority</skos:prefLabel>
    <skos:definition xml:lang="en">The lower tier of local government. Includes unitary authorities, districts, metropolitan districts and London boroughs.</skos:definition>
    <skos:altLabel xml:lang="en">Lower Tier Local Authority</skos:altLabel>
    <skos:broader rdf:resource="http://os.uk/vocabularies/collection/Boundaries" />
    <skos:broader rdf:resource="https://inspire.ec.europa.eu/metadata-codelist/TopicCategory/boundaries" />
    <skos:broader rdf:resource="https://inspire.ec.europa.eu/theme/au" />
    <skos:broader rdf:resource="http://inspire.ec.europa.eu/featureconcept/AdministrativeUnit" />
    <skos:inScheme rdf:resource="http://os.uk/vocabularies/ngd" />
  </rdf:Description>
  <rdf:Description rdf:about="http://os.uk/vocabularies/ngd/MaintenanceArea">
    <rdf:type rdf:resource="http://www.w3.org/2004/02/skos/core#Concept" />
    <skos:prefLabel xml:lang="en">Maintenance Area</skos:prefLabel>
    <skos:definition xml:lang="en">Indication of whether the highway is maintained by a Highways Authority, Local Highways Authority, Road Authority or privately, represented by an area feature.</skos:definition>
    <skos:altLabel xml:lang="en">Maintenance Area</skos:altLabel>
    <skos:broader rdf:resource="http://os.uk/vocabularies/collection/RAMI" />
    <skos:broader rdf:resource="https://inspire.ec.europa.eu/metadata-codelist/TopicCategory/transportation" />
    <skos:broader rdf:resource="https://inspire.ec.europa.eu/theme/tn" />
    <skos:inScheme rdf:resource="http://os.uk/vocabularies/ngd" />
  </rdf:Description>
  <rdf:Description rdf:about="http://os.uk/vocabularies/ngd/MaintenanceLine">
    <rdf:type rdf:resource="http://www.w3.org/2004/02/skos/core#Concept" />
    <skos:prefLabel xml:lang="en">Maintenance Line</skos:prefLabel>
    <skos:definition xml:lang="en">Indication of whether the highway is maintained by a Highways Authority, Local Highways Authority, Road Authority or privately, represented by a line feature.</skos:definition>
    <skos:altLabel xml:lang="en">Maintenance Line</skos:altLabel>
    <skos:broader rdf:resource="http://os.uk/vocabularies/collection/RAMI" />
    <skos:broader rdf:resource="https://inspire.ec.europa.eu/metadata-codelist/TopicCategory/transportation" />
    <skos:broader rdf:resource="https://inspire.ec.europa.eu/theme/tn" />
    <skos:broader rdf:resource="http://inspire.ec.europa.eu/featureconcept/MaintenanceAuthority" />
    <skos:inScheme rdf:resource="http://os.uk/vocabularies/ngd" />
  </rdf:Description>
  <rdf:Description rdf:about="http://os.uk/vocabularies/ngd/MaintenancePoint">
    <rdf:type rdf:resource="http://www.w3.org/2004/02/skos/core#Concept" />
    <skos:prefLabel xml:lang="en">Maintenance Point</skos:prefLabel>
    <skos:definition xml:lang="en">Indication of whether the highway is maintained by a Highways Authority, Local Highways Authority, Road Authority or privately, represented by a point feature.</skos:definition>
    <skos:altLabel xml:lang="en">Maintenance Point</skos:altLabel>
    <skos:broader rdf:resource="http://os.uk/vocabularies/collection/RAMI" />
    <skos:broader rdf:resource="https://inspire.ec.europa.eu/metadata-codelist/TopicCategory/transportation" />
    <skos:broader rdf:resource="https://inspire.ec.europa.eu/theme/tn" />
    <skos:broader rdf:resource="http://inspire.ec.europa.eu/featureconcept/MaintenanceAuthority" />
    <skos:inScheme rdf:resource="http://os.uk/vocabularies/ngd" />
  </rdf:Description>
  <rdf:Description rdf:about="http://os.uk/vocabularies/ngd/NamedArea">
    <rdf:type rdf:resource="http://www.w3.org/2004/02/skos/core#Concept" />
    <skos:prefLabel xml:lang="en">Named Area</skos:prefLabel>
    <skos:definition xml:lang="en">An area of land or water that has a name, that could not be captured in any of the other data themes.</skos:definition>
    <skos:altLabel xml:lang="en">Named Area</skos:altLabel>
    <skos:broader rdf:resource="http://os.uk/vocabularies/collection/Named-Features" />
    <skos:broader rdf:resource="https://inspire.ec.europa.eu/metadata-codelist/TopicCategory/location" />
    <skos:broader rdf:resource="https://inspire.ec.europa.eu/theme/gn" />
    <skos:broader rdf:resource="http://inspire.ec.europa.eu/featureconcept/NamedPlace" />
    <skos:inScheme rdf:resource="http://os.uk/vocabularies/ngd" />
  </rdf:Description>
  <rdf:Description rdf:about="http://os.uk/vocabularies/ngd/NamedPoint">
    <rdf:type rdf:resource="http://www.w3.org/2004/02/skos/core#Concept" />
    <skos:prefLabel xml:lang="en">Named Point</skos:prefLabel>
    <skos:definition xml:lang="en">An area of land or water that has a name, that could not be captured in any of the other data themes, represented as a point feature.</skos:definition>
    <skos:altLabel xml:lang="en">Named Point</skos:altLabel>
    <skos:broader rdf:resource="http://os.uk/vocabularies/collection/Named-Features" />
    <skos:broader rdf:resource="https://inspire.ec.europa.eu/metadata-codelist/TopicCategory/location" />
    <skos:broader rdf:resource="https://inspire.ec.europa.eu/theme/gn" />
    <skos:broader rdf:resource="http://inspire.ec.europa.eu/featureconcept/NamedPlace" />
    <skos:inScheme rdf:resource="http://os.uk/vocabularies/ngd" />
  </rdf:Description>
  <rdf:Description rdf:about="http://os.uk/vocabularies/ngd/NonAddressableObject">
    <rdf:type rdf:resource="http://www.w3.org/2004/02/skos/core#Concept" />
    <skos:prefLabel xml:lang="en">Non Addressable Object</skos:prefLabel>
    <skos:definition xml:lang="en">An address for a plot of land, a building or part of a building, or some other construction that cannot conceivably receive mail, deliveries or services.</skos:definition>
    <skos:altLabel xml:lang="en">Non Addressable Object</skos:altLabel>
    <skos:broader rdf:resource="http://os.uk/vocabularies/collection/GB-Address" />
    <skos:broader rdf:resource="http://os.uk/vocabularies/collection/Islands-Address" />
    <skos:broader rdf:resource="https://inspire.ec.europa.eu/metadata-codelist/TopicCategory/location" />
    <skos:broader rdf:resource="https://inspire.ec.europa.eu/theme/ad" />
    <skos:broader rdf:resource="http://inspire.ec.europa.eu/featureconcept/Address" />
    <skos:inScheme rdf:resource="http://os.uk/vocabularies/ngd" />
  </rdf:Description>
  <rdf:Description rdf:about="http://os.uk/vocabularies/ngd/ParishOrCommunity">
    <rdf:type rdf:resource="http://www.w3.org/2004/02/skos/core#Concept" />
    <skos:prefLabel xml:lang="en">Parish Or Community</skos:prefLabel>
    <skos:definition xml:lang="en">The smallest type of administrative area in England is the parish (aka 'civil parish'); the equivalent unit in Wales is the community. Scotland also has communities but their councils are generally a channel of opinion to other authorities rather than an administration in their own right.</skos:definition>
    <skos:altLabel xml:lang="en">Parish Or Community</skos:altLabel>
    <skos:broader rdf:resource="http://os.uk/vocabularies/collection/Boundaries" />
    <skos:broader rdf:resource="https://inspire.ec.europa.eu/metadata-codelist/TopicCategory/boundaries" />
    <skos:broader rdf:resource="https://inspire.ec.europa.eu/theme/au" />
    <skos:broader rdf:resource="http://inspire.ec.europa.eu/featureconcept/AdministrativeUnit" />
    <skos:inScheme rdf:resource="http://os.uk/vocabularies/ngd" />
  </rdf:Description>
  <rdf:Description rdf:about="http://os.uk/vocabularies/ngd/Path">
    <rdf:type rdf:resource="http://www.w3.org/2004/02/skos/core#Concept" />
    <skos:prefLabel xml:lang="en">Path</skos:prefLabel>
    <skos:definition xml:lang="en">A path with an accepted name.</skos:definition>
    <skos:broader rdf:resource="http://os.uk/vocabularies/collection/Transport-Network" />
    <skos:broader rdf:resource="https://inspire.ec.europa.eu/metadata-codelist/TopicCategory/transportation" />
    <skos:broader rdf:resource="https://inspire.ec.europa.eu/theme/tn" />
    <skos:broader rdf:resource="http://inspire.ec.europa.eu/featureconcept/Road" />
    <skos:inScheme rdf:resource="http://os.uk/vocabularies/ngd" />
  </rdf:Description>
  <rdf:Description rdf:about="http://os.uk/vocabularies/ngd/PathLink">
    <rdf:type rdf:resource="http://www.w3.org/2004/02/skos/core#Concept" />
    <skos:prefLabel xml:lang="en">Path Link</skos:prefLabel>
    <skos:definition xml:lang="en">A network representation of the general alignment of a route used by pedestrians.</skos:definition>
    <skos:altLabel xml:lang="en">Path Link</skos:altLabel>
    <skos:broader rdf:resource="http://os.uk/vocabularies/collection/Transport-Network" />
    <skos:broader rdf:resource="https://inspire.ec.europa.eu/metadata-codelist/TopicCategory/transportation" />
    <skos:broader rdf:resource="https://inspire.ec.europa.eu/theme/tn" />
    <skos:broader rdf:resource="http://inspire.ec.europa.eu/featureconcept/RoadLink" />
    <skos:inScheme rdf:resource="http://os.uk/vocabularies/ngd" />
  </rdf:Description>
  <rdf:Description rdf:about="http://os.uk/vocabularies/ngd/PathNode">
    <rdf:type rdf:resource="http://www.w3.org/2004/02/skos/core#Concept" />
    <skos:prefLabel xml:lang="en">Path Node</skos:prefLabel>
    <skos:definition xml:lang="en">The location where a path ends, is connected to two or more other paths or where a recorded attribute of a path changes.</skos:definition>
    <skos:altLabel xml:lang="en">Path Node</skos:altLabel>
    <skos:broader rdf:resource="http://os.uk/vocabularies/collection/Transport-Network" />
    <skos:broader rdf:resource="https://inspire.ec.europa.eu/metadata-codelist/TopicCategory/transportation" />
    <skos:broader rdf:resource="https://inspire.ec.europa.eu/theme/tn" />
    <skos:broader rdf:resource="http://inspire.ec.europa.eu/featureconcept/RoadNode" />
    <skos:inScheme rdf:resource="http://os.uk/vocabularies/ngd" />
  </rdf:Description>
  <rdf:Description rdf:about="http://os.uk/vocabularies/ngd/PollingDistrict">
    <rdf:type rdf:resource="http://www.w3.org/2004/02/skos/core#Concept" />
    <skos:prefLabel xml:lang="en">Polling District</skos:prefLabel>
    <skos:definition xml:lang="en">The geographical sub-division of an electoral area.</skos:definition>
    <skos:altLabel xml:lang="en">Polling District</skos:altLabel>
    <skos:broader rdf:resource="http://os.uk/vocabularies/collection/Boundaries" />
    <skos:broader rdf:resource="https://inspire.ec.europa.eu/metadata-codelist/TopicCategory/boundaries" />
    <skos:broader rdf:resource="https://inspire.ec.europa.eu/theme/au" />
    <skos:broader rdf:resource="http://inspire.ec.europa.eu/featureconcept/AdministrativeUnit" />
    <skos:inScheme rdf:resource="http://os.uk/vocabularies/ngd" />
  </rdf:Description>
  <rdf:Description rdf:about="http://os.uk/vocabularies/ngd/PreBuildAddress">
    <rdf:type rdf:resource="http://www.w3.org/2004/02/skos/core#Concept" />
    <skos:prefLabel xml:lang="en">Pre Build Address</skos:prefLabel>
    <skos:definition xml:lang="en">A new address for a plot of land, a building or part of a building, or some other construction that can conceivably receive mail, deliveries or services but has yet to be built or is under construction.</skos:definition>
    <skos:altLabel xml:lang="en">Pre Build Address</skos:altLabel>
    <skos:broader rdf:resource="http://os.uk/vocabularies/collection/GB-Address" />
    <skos:broader rdf:resource="http://os.uk/vocabularies/collection/Islands-Address" />
    <skos:broader rdf:resource="https://inspire.ec.europa.eu/metadata-codelist/TopicCategory/location" />
    <skos:broader rdf:resource="https://inspire.ec.europa.eu/theme/ad" />
    <skos:broader rdf:resource="http://inspire.ec.europa.eu/featureconcept/Address" />
    <skos:inScheme rdf:resource="http://os.uk/vocabularies/ngd" />
  </rdf:Description>
  <rdf:Description rdf:about="http://os.uk/vocabularies/ngd/Rail">
    <rdf:type rdf:resource="http://www.w3.org/2004/02/skos/core#Concept" />
    <skos:prefLabel xml:lang="en">Rail</skos:prefLabel>
    <skos:definition xml:lang="en">An area of Land exclusively associated with the rail transport.</skos:definition>
    <skos:broader rdf:resource="http://os.uk/vocabularies/collection/Transport-Network" />
    <skos:broader rdf:resource="https://inspire.ec.europa.eu/metadata-codelist/TopicCategory/transportation" />
    <skos:broader rdf:resource="https://inspire.ec.europa.eu/theme/tn" />
    <skos:broader rdf:resource="http://inspire.ec.europa.eu/featureconcept/RailwayArea" />
    <skos:inScheme rdf:resource="http://os.uk/vocabularies/ngd" />
  </rdf:Description>
  <rdf:Description rdf:about="http://os.uk/vocabularies/ngd/Region">
    <rdf:type rdf:resource="http://www.w3.org/2004/02/skos/core#Concept" />
    <skos:prefLabel xml:lang="en">Region</skos:prefLabel>
    <skos:definition xml:lang="en">Boundaries that were used to define Government Office Regions (GORs) in England, and are now used for statistical reporting and by the Boundary Commission for managing boundaries. Scotland and Wales have also been included to complement the product's GB coverage.</skos:definition>
    <skos:broader rdf:resource="http://os.uk/vocabularies/collection/Boundaries" />
    <skos:broader rdf:resource="https://inspire.ec.europa.eu/metadata-codelist/TopicCategory/boundaries" />
    <skos:broader rdf:resource="https://inspire.ec.europa.eu/theme/au" />
    <skos:broader rdf:resource="http://inspire.ec.europa.eu/featureconcept/AdministrativeUnit" />
    <skos:inScheme rdf:resource="http://os.uk/vocabularies/ngd" />
  </rdf:Description>
  <rdf:Description rdf:about="http://os.uk/vocabularies/ngd/RegionalAuthority">
    <rdf:type rdf:resource="http://www.w3.org/2004/02/skos/core#Concept" />
    <skos:prefLabel xml:lang="en">Regional Authority</skos:prefLabel>
    <skos:definition xml:lang="en">Currently contains a single feature: the Greater London Authority. In future can include combined authorities such as Greater Manchester.</skos:definition>
    <skos:altLabel xml:lang="en">Regional Authority</skos:altLabel>
    <skos:broader rdf:resource="http://os.uk/vocabularies/collection/Boundaries" />
    <skos:broader rdf:resource="https://inspire.ec.europa.eu/metadata-codelist/TopicCategory/boundaries" />
    <skos:broader rdf:resource="https://inspire.ec.europa.eu/theme/au" />
    <skos:broader rdf:resource="http://inspire.ec.europa.eu/featureconcept/AdministrativeUnit" />
    <skos:inScheme rdf:resource="http://os.uk/vocabularies/ngd" />
  </rdf:Description>
  <rdf:Description rdf:about="http://os.uk/vocabularies/ngd/ReinstatementArea">
    <rdf:type rdf:resource="http://www.w3.org/2004/02/skos/core#Concept" />
    <skos:prefLabel xml:lang="en">Reinstatement Area</skos:prefLabel>
    <skos:definition xml:lang="en">The standard to which the highway must be restored to following street works, represented by an area feature.</skos:definition>
    <skos:altLabel xml:lang="en">Reinstatement Area</skos:altLabel>
    <skos:broader rdf:resource="http://os.uk/vocabularies/collection/RAMI" />
    <skos:broader rdf:resource="https://inspire.ec.europa.eu/metadata-codelist/TopicCategory/transportation" />
    <skos:broader rdf:resource="https://inspire.ec.europa.eu/theme/tn" />
    <skos:inScheme rdf:resource="http://os.uk/vocabularies/ngd" />
  </rdf:Description>
  <rdf:Description rdf:about="http://os.uk/vocabularies/ngd/ReinstatementLine">
    <rdf:type rdf:resource="http://www.w3.org/2004/02/skos/core#Concept" />
    <skos:prefLabel xml:lang="en">Reinstatement Line</skos:prefLabel>
    <skos:definition xml:lang="en">The standard to which the highway must be restored to following street works, represented by a line feature.</skos:definition>
    <skos:altLabel xml:lang="en">Reinstatement Line</skos:altLabel>
    <skos:broader rdf:resource="http://os.uk/vocabularies/collection/RAMI" />
    <skos:broader rdf:resource="https://inspire.ec.europa.eu/metadata-codelist/TopicCategory/transportation" />
    <skos:broader rdf:resource="https://inspire.ec.europa.eu/theme/tn" />
    <skos:inScheme rdf:resource="http://os.uk/vocabularies/ngd" />
  </rdf:Description>
  <rdf:Description rdf:about="http://os.uk/vocabularies/ngd/ReinstatementPoint">
    <rdf:type rdf:resource="http://www.w3.org/2004/02/skos/core#Concept" />
    <skos:prefLabel xml:lang="en">Reinstatement Point</skos:prefLabel>
    <skos:definition xml:lang="en">The standard to which the highway must be restored to following street works, represented by a point feature.</skos:definition>
    <skos:altLabel xml:lang="en">Reinstatement Point</skos:altLabel>
    <skos:broader rdf:resource="http://os.uk/vocabularies/collection/RAMI" />
    <skos:broader rdf:resource="https://inspire.ec.europa.eu/metadata-codelist/TopicCategory/transportation" />
    <skos:broader rdf:resource="https://inspire.ec.europa.eu/theme/tn" />
    <skos:inScheme rdf:resource="http://os.uk/vocabularies/ngd" />
  </rdf:Description>
  <rdf:Description rdf:about="http://os.uk/vocabularies/ngd/Restriction">
    <rdf:type rdf:resource="http://www.w3.org/2004/02/skos/core#Concept" />
    <skos:prefLabel xml:lang="en">Restriction</skos:prefLabel>
    <skos:definition xml:lang="en">A restriction based on vehicular access to a highway or a restriction on vehicular manoeuvre.</skos:definition>
    <skos:broader rdf:resource="http://os.uk/vocabularies/collection/RAMI" />
    <skos:broader rdf:resource="https://inspire.ec.europa.eu/metadata-codelist/TopicCategory/transportation" />
    <skos:broader rdf:resource="https://inspire.ec.europa.eu/theme/tn" />
    <skos:exactMatch rdf:resource="http://inspire.ec.europa.eu/featureconcept/RestrictionForVehicles" />
    <skos:inScheme rdf:resource="http://os.uk/vocabularies/ngd" />
  </rdf:Description>
  <rdf:Description rdf:about="http://os.uk/vocabularies/ngd/Road">
    <rdf:type rdf:resource="http://www.w3.org/2004/02/skos/core#Concept" />
    <skos:prefLabel xml:lang="en">Road</skos:prefLabel>
    <skos:definition xml:lang="en">A road with an accepted name or official government number.</skos:definition>
    <skos:broader rdf:resource="http://os.uk/vocabularies/collection/Transport-Network" />
    <skos:broader rdf:resource="https://inspire.ec.europa.eu/metadata-codelist/TopicCategory/transportation" />
    <skos:broader rdf:resource="https://inspire.ec.europa.eu/theme/tn" />
    <skos:exactMatch rdf:resource="http://inspire.ec.europa.eu/featureconcept/Road" />
    <skos:inScheme rdf:resource="http://os.uk/vocabularies/ngd" />
  </rdf:Description>
  <rdf:Description rdf:about="http://os.uk/vocabularies/ngd/RoadJunction">
    <rdf:type rdf:resource="http://www.w3.org/2004/02/skos/core#Concept" />
    <skos:prefLabel xml:lang="en">Road Junction</skos:prefLabel>
    <skos:definition xml:lang="en">An intersection of roads with an accepted name or official government number.</skos:definition>
    <skos:altLabel xml:lang="en">Road Junction</skos:altLabel>
    <skos:broader rdf:resource="http://os.uk/vocabularies/collection/Transport-Network" />
    <skos:broader rdf:resource="https://inspire.ec.europa.eu/metadata-codelist/TopicCategory/transportation" />
    <skos:broader rdf:resource="https://inspire.ec.europa.eu/theme/tn" />
    <skos:broader rdf:resource="http://inspire.ec.europa.eu/featureconcept/RoadNode" />
    <skos:inScheme rdf:resource="http://os.uk/vocabularies/ngd" />
  </rdf:Description>
  <rdf:Description rdf:about="http://os.uk/vocabularies/ngd/RoadLine">
    <rdf:type rdf:resource="http://www.w3.org/2004/02/skos/core#Concept" />
    <skos:prefLabel xml:lang="en">Road Line</skos:prefLabel>
    <skos:definition xml:lang="en">A linear feature associated with the passage of vehicles, pedestrians and animals being ridden or led.</skos:definition>
    <skos:altLabel xml:lang="en">Road Line</skos:altLabel>
    <skos:broader rdf:resource="http://os.uk/vocabularies/collection/Transport-Features" />
    <skos:broader rdf:resource="https://inspire.ec.europa.eu/metadata-codelist/TopicCategory/transportation" />
    <skos:broader rdf:resource="https://inspire.ec.europa.eu/theme/tn" />
    <skos:broader rdf:resource="http://inspire.ec.europa.eu/featureconcept/RoadLinkSequence" />
    <skos:inScheme rdf:resource="http://os.uk/vocabularies/ngd" />
  </rdf:Description>
  <rdf:Description rdf:about="http://os.uk/vocabularies/ngd/RoadLink">
    <rdf:type rdf:resource="http://www.w3.org/2004/02/skos/core#Concept" />
    <skos:prefLabel xml:lang="en">Road Link</skos:prefLabel>
    <skos:definition xml:lang="en">A network representation of the general alignment of a route used by vehicles and potentially other users.</skos:definition>
    <skos:altLabel xml:lang="en">Road Link</skos:altLabel>
    <skos:broader rdf:resource="http://os.uk/vocabularies/collection/Transport-Network" />
    <skos:broader rdf:resource="https://inspire.ec.europa.eu/metadata-codelist/TopicCategory/transportation" />
    <skos:broader rdf:resource="https://inspire.ec.europa.eu/theme/tn" />
    <skos:exactMatch rdf:resource="http://inspire.ec.europa.eu/featureconcept/RoadLink" />
    <skos:inScheme rdf:resource="http://os.uk/vocabularies/ngd" />
  </rdf:Description>
  <rdf:Description rdf:about="http://os.uk/vocabularies/ngd/RoadNode">
    <rdf:type rdf:resource="http://www.w3.org/2004/02/skos/core#Concept" />
    <skos:prefLabel xml:lang="en">Road Node</skos:prefLabel>
    <skos:definition xml:lang="en">The location where a road ends, is connected to two or more other paths or where a recorded attribute of a road changes.</skos:definition>
    <skos:altLabel xml:lang="en">Road Node</skos:altLabel>
    <skos:broader rdf:resource="http://os.uk/vocabularies/collection/Transport-Network" />
    <skos:broader rdf:resource="https://inspire.ec.europa.eu/metadata-codelist/TopicCategory/transportation" />
    <skos:broader rdf:resource="https://inspire.ec.europa.eu/theme/tn" />
    <skos:exactMatch rdf:resource="http://inspire.ec.europa.eu/featureconcept/RoadNode" />
    <skos:inScheme rdf:resource="http://os.uk/vocabularies/ngd" />
  </rdf:Description>
  <rdf:Description rdf:about="http://os.uk/vocabularies/ngd/RoadTrackOrPath">
    <rdf:type rdf:resource="http://www.w3.org/2004/02/skos/core#Concept" />
    <skos:prefLabel xml:lang="en">Road Track Or Path</skos:prefLabel>
    <skos:definition xml:lang="en">An area of Land associated with the passage of vehicles, pedestrians and animals being ridden or led.</skos:definition>
    <skos:altLabel xml:lang="en">Road Track Or Path</skos:altLabel>
    <skos:broader rdf:resource="http://os.uk/vocabularies/collection/Transport-Features" />
    <skos:broader rdf:resource="https://inspire.ec.europa.eu/metadata-codelist/TopicCategory/transportation" />
    <skos:broader rdf:resource="https://inspire.ec.europa.eu/theme/tn" />
    <skos:broader rdf:resource="http://inspire.ec.europa.eu/featureconcept/RoadLinkSequence" />
    <skos:inScheme rdf:resource="http://os.uk/vocabularies/ngd" />
  </rdf:Description>
  <rdf:Description rdf:about="http://os.uk/vocabularies/ngd/RoutingHazard">
    <rdf:type rdf:resource="http://www.w3.org/2004/02/skos/core#Concept" />
    <skos:prefLabel xml:lang="en">Routing Hazard</skos:prefLabel>
    <skos:definition xml:lang="en">A location where a threat is imposed and caution should be taken with relation to the highway network.</skos:definition>
    <skos:altLabel xml:lang="en">Routing Hazard</skos:altLabel>
    <skos:broader rdf:resource="http://os.uk/vocabularies/collection/RAMI" />
    <skos:broader rdf:resource="https://inspire.ec.europa.eu/metadata-codelist/TopicCategory/transportation" />
    <skos:broader rdf:resource="https://inspire.ec.europa.eu/theme/tn" />
    <skos:inScheme rdf:resource="http://os.uk/vocabularies/ngd" />
  </rdf:Description>
  <rdf:Description rdf:about="http://os.uk/vocabularies/ngd/RoutingStructure">
    <rdf:type rdf:resource="http://www.w3.org/2004/02/skos/core#Concept" />
    <skos:prefLabel xml:lang="en">Routing Structure</skos:prefLabel>
    <skos:definition xml:lang="en">A built feature with relation to the highway network.</skos:definition>
    <skos:altLabel xml:lang="en">Routing Structure</skos:altLabel>
    <skos:broader rdf:resource="http://os.uk/vocabularies/collection/RAMI" />
    <skos:broader rdf:resource="https://inspire.ec.europa.eu/metadata-codelist/TopicCategory/transportation" />
    <skos:broader rdf:resource="https://inspire.ec.europa.eu/theme/tn" />
    <skos:inScheme rdf:resource="http://os.uk/vocabularies/ngd" />
  </rdf:Description>
  <rdf:Description rdf:about="http://os.uk/vocabularies/ngd/Site">
    <rdf:type rdf:resource="http://www.w3.org/2004/02/skos/core#Concept" />
    <skos:prefLabel xml:lang="en">Site</skos:prefLabel>
    <skos:definition xml:lang="en">A multi-surface feature representing the extent of certain types of function or activity.</skos:definition>
    <skos:broader rdf:resource="http://os.uk/vocabularies/collection/Land-Use-Features" />
    <skos:broader rdf:resource="https://inspire.ec.europa.eu/metadata-codelist/TopicCategory/location" />
    <skos:inScheme rdf:resource="http://os.uk/vocabularies/ngd" />
  </rdf:Description>
  <rdf:Description rdf:about="http://os.uk/vocabularies/ngd/SiteAccessLocation">
    <rdf:type rdf:resource="http://www.w3.org/2004/02/skos/core#Concept" />
    <skos:prefLabel xml:lang="en">Site Access Location</skos:prefLabel>
    <skos:definition xml:lang="en">A point feature representing the accepted and/or maintained locations where pedestrians and/or vehicles can enter or exit a site.</skos:definition>
    <skos:altLabel xml:lang="en">Site Access Location</skos:altLabel>
    <skos:broader rdf:resource="http://os.uk/vocabularies/collection/Land-Use-Features" />
    <skos:broader rdf:resource="https://inspire.ec.europa.eu/metadata-codelist/TopicCategory/transportation" />
    <skos:inScheme rdf:resource="http://os.uk/vocabularies/ngd" />
  </rdf:Description>
  <rdf:Description rdf:about="http://os.uk/vocabularies/ngd/SiteRoutingPoint">
    <rdf:type rdf:resource="http://www.w3.org/2004/02/skos/core#Concept" />
    <skos:prefLabel xml:lang="en">Site Routing Point</skos:prefLabel>
    <skos:definition xml:lang="en">The location on the road network that provides entry or exit into a site for vehicles.</skos:definition>
    <skos:altLabel xml:lang="en">Site Routing Point</skos:altLabel>
    <skos:broader rdf:resource="http://os.uk/vocabularies/collection/Land-Use-Features" />
    <skos:broader rdf:resource="https://inspire.ec.europa.eu/metadata-codelist/TopicCategory/transportation" />
    <skos:inScheme rdf:resource="http://os.uk/vocabularies/ngd" />
  </rdf:Description>
  <rdf:Description rdf:about="http://os.uk/vocabularies/ngd/SpecialDesignationArea">
    <rdf:type rdf:resource="http://www.w3.org/2004/02/skos/core#Concept" />
    <skos:prefLabel xml:lang="en">Special Designation Area</skos:prefLabel>
    <skos:definition xml:lang="en">A description applied to a highway to protect it during Street or Road Works, represented by an area feature.</skos:definition>
    <skos:altLabel xml:lang="en">Special Designation Area</skos:altLabel>
    <skos:broader rdf:resource="http://os.uk/vocabularies/collection/RAMI" />
    <skos:broader rdf:resource="https://inspire.ec.europa.eu/metadata-codelist/TopicCategory/transportation" />
    <skos:broader rdf:resource="https://inspire.ec.europa.eu/theme/tn" />
    <skos:inScheme rdf:resource="http://os.uk/vocabularies/ngd" />
  </rdf:Description>
  <rdf:Description rdf:about="http://os.uk/vocabularies/ngd/SpecialDesignationLine">
    <rdf:type rdf:resource="http://www.w3.org/2004/02/skos/core#Concept" />
    <skos:prefLabel xml:lang="en">Special Designation Line</skos:prefLabel>
    <skos:definition xml:lang="en">A description applied to a highway to protect it during Street or Road Works, represented by a line feature.</skos:definition>
    <skos:altLabel xml:lang="en">Special Designation Line</skos:altLabel>
    <skos:broader rdf:resource="http://os.uk/vocabularies/collection/RAMI" />
    <skos:broader rdf:resource="https://inspire.ec.europa.eu/metadata-codelist/TopicCategory/transportation" />
    <skos:broader rdf:resource="https://inspire.ec.europa.eu/theme/tn" />
    <skos:inScheme rdf:resource="http://os.uk/vocabularies/ngd" />
  </rdf:Description>
  <rdf:Description rdf:about="http://os.uk/vocabularies/ngd/SpecialDesignationPoint">
    <rdf:type rdf:resource="http://www.w3.org/2004/02/skos/core#Concept" />
    <skos:prefLabel xml:lang="en">Special Designation Point</skos:prefLabel>
    <skos:definition xml:lang="en">A description applied to a highway to protect it during Street or Road Works, represented by a point feature.</skos:definition>
    <skos:altLabel xml:lang="en">Special Designation Point</skos:altLabel>
    <skos:broader rdf:resource="http://os.uk/vocabularies/collection/RAMI" />
    <skos:broader rdf:resource="https://inspire.ec.europa.eu/metadata-codelist/TopicCategory/transportation" />
    <skos:broader rdf:resource="https://inspire.ec.europa.eu/theme/tn" />
    <skos:inScheme rdf:resource="http://os.uk/vocabularies/ngd" />
  </rdf:Description>
  <rdf:Description rdf:about="http://os.uk/vocabularies/ngd/Street">
    <rdf:type rdf:resource="http://www.w3.org/2004/02/skos/core#Concept" />
    <skos:prefLabel xml:lang="en">Street</skos:prefLabel>
    <skos:definition xml:lang="en">Any road, footway, path, cycletrack, track or passageway that has been uniquely identified by the local Highway Authority.</skos:definition>
    <skos:broader rdf:resource="http://os.uk/vocabularies/collection/Transport-Network" />
    <skos:broader rdf:resource="https://inspire.ec.europa.eu/metadata-codelist/TopicCategory/transportation" />
    <skos:broader rdf:resource="https://inspire.ec.europa.eu/theme/tn" />
    <skos:broader rdf:resource="http://inspire.ec.europa.eu/featureconcept/Road" />
    <skos:inScheme rdf:resource="http://os.uk/vocabularies/ngd" />
  </rdf:Description>
  <rdf:Description rdf:about="http://os.uk/vocabularies/ngd/StreetAddress">
    <rdf:type rdf:resource="http://www.w3.org/2004/02/skos/core#Concept" />
    <skos:prefLabel xml:lang="en">Street Address</skos:prefLabel>
    <skos:definition xml:lang="en">Any road, footway, path, cycletrack, track or passageway that has been uniquely identified by the local Highway Authority and has an addressable object.</skos:definition>
    <skos:altLabel xml:lang="en">Street Address</skos:altLabel>
    <skos:broader rdf:resource="http://os.uk/vocabularies/collection/GB-Address" />
    <skos:broader rdf:resource="http://os.uk/vocabularies/collection/Islands-Address" />
    <skos:broader rdf:resource="https://inspire.ec.europa.eu/metadata-codelist/TopicCategory/location" />
    <skos:broader rdf:resource="https://inspire.ec.europa.eu/theme/ad" />
    <skos:broader rdf:resource="http://inspire.ec.europa.eu/featureconcept/ThoroughfareName" />
    <skos:inScheme rdf:resource="http://os.uk/vocabularies/ngd" />
  </rdf:Description>
  <rdf:Description rdf:about="http://os.uk/vocabularies/ngd/Structure">
    <rdf:type rdf:resource="http://www.w3.org/2004/02/skos/core#Concept" />
    <skos:prefLabel xml:lang="en">Structure</skos:prefLabel>
    <skos:definition xml:lang="en">A manmade construction that is not a building.</skos:definition>
    <skos:broader rdf:resource="http://os.uk/vocabularies/collection/Structure-Features" />
    <skos:broader rdf:resource="https://inspire.ec.europa.eu/metadata-codelist/TopicCategory/structure" />
    <skos:broader rdf:resource="https://inspire.ec.europa.eu/theme/bu" />
    <skos:inScheme rdf:resource="http://os.uk/vocabularies/ngd" />
  </rdf:Description>
  <rdf:Description rdf:about="http://os.uk/vocabularies/ngd/StructureLine">
    <rdf:type rdf:resource="http://www.w3.org/2004/02/skos/core#Concept" />
    <skos:prefLabel xml:lang="en">Structure Line</skos:prefLabel>
    <skos:definition xml:lang="en">A linear freestanding manmade construction that is not a building nor wide enough to capture as a Structure.</skos:definition>
    <skos:altLabel xml:lang="en">Structure Line</skos:altLabel>
    <skos:broader rdf:resource="http://os.uk/vocabularies/collection/Structure-Features" />
    <skos:broader rdf:resource="https://inspire.ec.europa.eu/metadata-codelist/TopicCategory/structure" />
    <skos:broader rdf:resource="https://inspire.ec.europa.eu/theme/bu" />
    <skos:inScheme rdf:resource="http://os.uk/vocabularies/ngd" />
  </rdf:Description>
  <rdf:Description rdf:about="http://os.uk/vocabularies/ngd/StructurePoint">
    <rdf:type rdf:resource="http://www.w3.org/2004/02/skos/core#Concept" />
    <skos:prefLabel xml:lang="en">Structure Point</skos:prefLabel>
    <skos:definition xml:lang="en">A freestanding manmade construction that is not a building and that is less than 4m square but that is considered to be of sufficient interest to be captured.</skos:definition>
    <skos:altLabel xml:lang="en">Structure Point</skos:altLabel>
    <skos:broader rdf:resource="http://os.uk/vocabularies/collection/Structure-Features" />
    <skos:broader rdf:resource="https://inspire.ec.europa.eu/metadata-codelist/TopicCategory/structure" />
    <skos:broader rdf:resource="https://inspire.ec.europa.eu/theme/bu" />
    <skos:inScheme rdf:resource="http://os.uk/vocabularies/ngd" />
  </rdf:Description>
  <rdf:Description rdf:about="http://os.uk/vocabularies/ngd/TidalBoundary">
    <rdf:type rdf:resource="http://www.w3.org/2004/02/skos/core#Concept" />
    <skos:prefLabel xml:lang="en">Tidal Boundary</skos:prefLabel>
    <skos:definition xml:lang="en">The alignment of the limit of tidal water at specific states of the tide.</skos:definition>
    <skos:altLabel xml:lang="en">Tidal Boundary</skos:altLabel>
    <skos:broader rdf:resource="http://os.uk/vocabularies/collection/Water-Features" />
    <skos:broader rdf:resource="https://inspire.ec.europa.eu/metadata-codelist/TopicCategory/oceans" />
    <skos:broader rdf:resource="https://inspire.ec.europa.eu/theme/hy" />
    <skos:broader rdf:resource="http://inspire.ec.europa.eu/featureconcept/LandWaterBoundary" />
    <skos:inScheme rdf:resource="http://os.uk/vocabularies/ngd" />
  </rdf:Description>
  <rdf:Description rdf:about="http://os.uk/vocabularies/ngd/UpperTierLocalAuthority">
    <rdf:type rdf:resource="http://www.w3.org/2004/02/skos/core#Concept" />
    <skos:prefLabel xml:lang="en">Upper Tier Local Authority</skos:prefLabel>
    <skos:definition xml:lang="en">The upper tier of local government. Includes unitary authorities, non-metropolitan counties, metropolitan districts and London boroughs.</skos:definition>
    <skos:altLabel xml:lang="en">Upper Tier Local Authority</skos:altLabel>
    <skos:broader rdf:resource="http://os.uk/vocabularies/collection/Boundaries" />
    <skos:broader rdf:resource="https://inspire.ec.europa.eu/metadata-codelist/TopicCategory/boundaries" />
    <skos:broader rdf:resource="https://inspire.ec.europa.eu/theme/au" />
    <skos:broader rdf:resource="http://inspire.ec.europa.eu/featureconcept/AdministrativeUnit" />
    <skos:inScheme rdf:resource="http://os.uk/vocabularies/ngd" />
  </rdf:Description>
  <rdf:Description rdf:about="http://os.uk/vocabularies/ngd/Ward">
    <rdf:type rdf:resource="http://www.w3.org/2004/02/skos/core#Concept" />
    <skos:prefLabel xml:lang="en">Ward</skos:prefLabel>
    <skos:definition xml:lang="en">Electoral wards/divisions are the key building blocks of UK administrative geography. They are the spatial units used to elect local government councilors in metropolitan and non-metropolitan districts, unitary authorities and the London boroughs in England; unitary authorities in Wales and council areas in Scotland. Electoral wards are specifically used in communities, districts, London boroughs, metropolitan districts, Scottish unitary authorities and some English unitary authorities.</skos:definition>
    <skos:broader rdf:resource="http://os.uk/vocabularies/collection/Boundaries" />
    <skos:broader rdf:resource="https://inspire.ec.europa.eu/metadata-codelist/TopicCategory/boundaries" />
    <skos:broader rdf:resource="https://inspire.ec.europa.eu/theme/au" />
    <skos:broader rdf:resource="http://inspire.ec.europa.eu/featureconcept/AdministrativeUnit" />
    <skos:inScheme rdf:resource="http://os.uk/vocabularies/ngd" />
  </rdf:Description>
  <rdf:Description rdf:about="http://os.uk/vocabularies/ngd/Water">
    <rdf:type rdf:resource="http://www.w3.org/2004/02/skos/core#Concept" />
    <skos:prefLabel xml:lang="en">Water</skos:prefLabel>
    <skos:definition xml:lang="en">An area of permanent water.</skos:definition>
    <skos:broader rdf:resource="http://os.uk/vocabularies/collection/Water-Features" />
    <skos:broader rdf:resource="https://inspire.ec.europa.eu/metadata-codelist/TopicCategory/inlandWaters" />
    <skos:broader rdf:resource="https://inspire.ec.europa.eu/theme/hy" />
    <skos:broader rdf:resource="http://inspire.ec.europa.eu/featureconcept/StandingWater" />
    <skos:inScheme rdf:resource="http://os.uk/vocabularies/ngd" />
  </rdf:Description>
  <rdf:Description rdf:about="http://os.uk/vocabularies/ngd/WaterLink">
    <rdf:type rdf:resource="http://www.w3.org/2004/02/skos/core#Concept" />
    <skos:prefLabel xml:lang="en">Water Link</skos:prefLabel>
    <skos:definition xml:lang="en">A network representation of the general alignment of areas of permanent water where they are connected.</skos:definition>
    <skos:altLabel xml:lang="en">Water Link</skos:altLabel>
    <skos:broader rdf:resource="http://os.uk/vocabularies/collection/Water-Network" />
    <skos:broader rdf:resource="https://inspire.ec.europa.eu/metadata-codelist/TopicCategory/inlandWaters" />
    <skos:broader rdf:resource="https://inspire.ec.europa.eu/theme/hy" />
    <skos:exactMatch rdf:resource="http://inspire.ec.europa.eu/featureconcept/WatercourseLink" />
    <skos:inScheme rdf:resource="http://os.uk/vocabularies/ngd" />
  </rdf:Description>
  <rdf:Description rdf:about="http://os.uk/vocabularies/ngd/WaterLinkSet">
    <rdf:type rdf:resource="http://www.w3.org/2004/02/skos/core#Concept" />
    <skos:prefLabel xml:lang="en">Water Link Set</skos:prefLabel>
    <skos:definition xml:lang="en">A body of water with an accepted name that the water network flows through.</skos:definition>
    <skos:altLabel xml:lang="en">Water Link Set</skos:altLabel>
    <skos:broader rdf:resource="http://os.uk/vocabularies/collection/Water-Network" />
    <skos:broader rdf:resource="https://inspire.ec.europa.eu/metadata-codelist/TopicCategory/inlandWaters" />
    <skos:broader rdf:resource="https://inspire.ec.europa.eu/theme/hy" />
    <skos:broader rdf:resource="http://inspire.ec.europa.eu/featureconcept/Watercourse" />
    <skos:inScheme rdf:resource="http://os.uk/vocabularies/ngd" />
  </rdf:Description>
  <rdf:Description rdf:about="http://os.uk/vocabularies/ngd/WaterNode">
    <rdf:type rdf:resource="http://www.w3.org/2004/02/skos/core#Concept" />
    <skos:prefLabel xml:lang="en">Water Node</skos:prefLabel>
    <skos:definition xml:lang="en">The location where a connected area of permanent water ends, is connected to two or more other areas of permanent water or where a recorded attribute changes.</skos:definition>
    <skos:altLabel xml:lang="en">Water Node</skos:altLabel>
    <skos:broader rdf:resource="http://os.uk/vocabularies/collection/Water-Network" />
    <skos:broader rdf:resource="https://inspire.ec.europa.eu/metadata-codelist/TopicCategory/inlandWaters" />
    <skos:broader rdf:resource="https://inspire.ec.europa.eu/theme/hy" />
    <skos:exactMatch rdf:resource="http://inspire.ec.europa.eu/featureconcept/HydroNode" />
    <skos:inScheme rdf:resource="http://os.uk/vocabularies/ngd" />
  </rdf:Description>
  <rdf:Description rdf:about="http://os.uk/vocabularies/ngd/WaterPoint">
    <rdf:type rdf:resource="http://www.w3.org/2004/02/skos/core#Concept" />
    <skos:prefLabel xml:lang="en">Water Point</skos:prefLabel>
    <skos:definition xml:lang="en">A feature associated with permanent water that is too small to be captured as a Water feature but that is considered to be of sufficient interest to be captured.</skos:definition>
    <skos:altLabel xml:lang="en">Water Point</skos:altLabel>
    <skos:broader rdf:resource="http://os.uk/vocabularies/collection/Water-Features" />
    <skos:broader rdf:resource="https://inspire.ec.europa.eu/metadata-codelist/TopicCategory/inlandWaters" />
    <skos:broader rdf:resource="https://inspire.ec.europa.eu/theme/hy" />
    <skos:inScheme rdf:resource="http://os.uk/vocabularies/ngd" />
  </rdf:Description>
  <rdf:Description rdf:about="http://os.uk/vocabularies/ngd/WestminsterConstituency">
    <rdf:type rdf:resource="http://www.w3.org/2004/02/skos/core#Concept" />
    <skos:prefLabel xml:lang="en">Westminster Constituency</skos:prefLabel>
    <skos:definition xml:lang="en">Westminster parliamentary constituencies are used to elect members to the UK Parliament in Westminster, London.</skos:definition>
    <skos:altLabel xml:lang="en">Westminster Constituency</skos:altLabel>
    <skos:broader rdf:resource="http://os.uk/vocabularies/collection/Boundaries" />
    <skos:broader rdf:resource="https://inspire.ec.europa.eu/metadata-codelist/TopicCategory/boundaries" />
    <skos:broader rdf:resource="https://inspire.ec.europa.eu/theme/au" />
    <skos:broader rdf:resource="http://inspire.ec.europa.eu/featureconcept/AdministrativeUnit" />
    <skos:inScheme rdf:resource="http://os.uk/vocabularies/ngd" />
  </rdf:Description>
  <rdf:Description rdf:about="http://os.uk/vocabularies/collection/Boundaries">
    <skos:narrower rdf:resource="http://os.uk/vocabularies/ngd/BoundaryHighWaterMark" />
    <skos:narrower rdf:resource="http://os.uk/vocabularies/ngd/CeremonialCounty" />
    <skos:narrower rdf:resource="http://os.uk/vocabularies/ngd/Country" />
    <skos:narrower rdf:resource="http://os.uk/vocabularies/ngd/DevolvedParliamentConstituency" />
    <skos:narrower rdf:resource="http://os.uk/vocabularies/ngd/DevolvedParliamentElectoralRegion" />
    <skos:narrower rdf:resource="http://os.uk/vocabularies/ngd/ElectoralDivision" />
    <skos:narrower rdf:resource="http://os.uk/vocabularies/ngd/GLAAssemblyConstituency" />
    <skos:narrower rdf:resource="http://os.uk/vocabularies/ngd/HistoricCounty" />
    <skos:narrower rdf:resource="http://os.uk/vocabularies/ngd/HistoricEuropeanRegion" />
    <skos:narrower rdf:resource="http://os.uk/vocabularies/ngd/LowerTierLocalAuthority" />
    <skos:narrower rdf:resource="http://os.uk/vocabularies/ngd/ParishOrCommunity" />
    <skos:narrower rdf:resource="http://os.uk/vocabularies/ngd/PollingDistrict" />
    <skos:narrower rdf:resource="http://os.uk/vocabularies/ngd/Region" />
    <skos:narrower rdf:resource="http://os.uk/vocabularies/ngd/RegionalAuthority" />
    <skos:narrower rdf:resource="http://os.uk/vocabularies/ngd/UpperTierLocalAuthority" />
    <skos:narrower rdf:resource="http://os.uk/vocabularies/ngd/Ward" />
    <skos:narrower rdf:resource="http://os.uk/vocabularies/ngd/WestminsterConstituency" />
  </rdf:Description>
  <rdf:Description rdf:about="https://inspire.ec.europa.eu/metadata-codelist/TopicCategory/boundaries">
    <skos:narrower rdf:resource="http://os.uk/vocabularies/ngd/BoundaryHighWaterMark" />
    <skos:narrower rdf:resource="http://os.uk/vocabularies/ngd/CeremonialCounty" />
    <skos:narrower rdf:resource="http://os.uk/vocabularies/ngd/Country" />
    <skos:narrower rdf:resource="http://os.uk/vocabularies/ngd/DevolvedParliamentConstituency" />
    <skos:narrower rdf:resource="http://os.uk/vocabularies/ngd/DevolvedParliamentElectoralRegion" />
    <skos:narrower rdf:resource="http://os.uk/vocabularies/ngd/ElectoralDivision" />
    <skos:narrower rdf:resource="http://os.uk/vocabularies/ngd/GLAAssemblyConstituency" />
    <skos:narrower rdf:resource="http://os.uk/vocabularies/ngd/HistoricCounty" />
    <skos:narrower rdf:resource="http://os.uk/vocabularies/ngd/HistoricEuropeanRegion" />
    <skos:narrower rdf:resource="http://os.uk/vocabularies/ngd/LowerTierLocalAuthority" />
    <skos:narrower rdf:resource="http://os.uk/vocabularies/ngd/ParishOrCommunity" />
    <skos:narrower rdf:resource="http://os.uk/vocabularies/ngd/PollingDistrict" />
    <skos:narrower rdf:resource="http://os.uk/vocabularies/ngd/Region" />
    <skos:narrower rdf:resource="http://os.uk/vocabularies/ngd/RegionalAuthority" />
    <skos:narrower rdf:resource="http://os.uk/vocabularies/ngd/UpperTierLocalAuthority" />
    <skos:narrower rdf:resource="http://os.uk/vocabularies/ngd/Ward" />
    <skos:narrower rdf:resource="http://os.uk/vocabularies/ngd/WestminsterConstituency" />
  </rdf:Description>
  <rdf:Description rdf:about="https://inspire.ec.europa.eu/theme/au">
    <skos:narrower rdf:resource="http://os.uk/vocabularies/ngd/BoundaryHighWaterMark" />
    <skos:narrower rdf:resource="http://os.uk/vocabularies/ngd/CeremonialCounty" />
    <skos:narrower rdf:resource="http://os.uk/vocabularies/ngd/Country" />
    <skos:narrower rdf:resource="http://os.uk/vocabularies/ngd/DevolvedParliamentConstituency" />
    <skos:narrower rdf:resource="http://os.uk/vocabularies/ngd/DevolvedParliamentElectoralRegion" />
    <skos:narrower rdf:resource="http://os.uk/vocabularies/ngd/ElectoralDivision" />
    <skos:narrower rdf:resource="http://os.uk/vocabularies/ngd/GLAAssemblyConstituency" />
    <skos:narrower rdf:resource="http://os.uk/vocabularies/ngd/HistoricCounty" />
    <skos:narrower rdf:resource="http://os.uk/vocabularies/ngd/HistoricEuropeanRegion" />
    <skos:narrower rdf:resource="http://os.uk/vocabularies/ngd/LowerTierLocalAuthority" />
    <skos:narrower rdf:resource="http://os.uk/vocabularies/ngd/ParishOrCommunity" />
    <skos:narrower rdf:resource="http://os.uk/vocabularies/ngd/PollingDistrict" />
    <skos:narrower rdf:resource="http://os.uk/vocabularies/ngd/Region" />
    <skos:narrower rdf:resource="http://os.uk/vocabularies/ngd/RegionalAuthority" />
    <skos:narrower rdf:resource="http://os.uk/vocabularies/ngd/UpperTierLocalAuthority" />
    <skos:narrower rdf:resource="http://os.uk/vocabularies/ngd/Ward" />
    <skos:narrower rdf:resource="http://os.uk/vocabularies/ngd/WestminsterConstituency" />
  </rdf:Description>
  <rdf:Description rdf:about="http://inspire.ec.europa.eu/featureconcept/AdministrativeBoundary">
    <skos:narrower rdf:resource="http://os.uk/vocabularies/ngd/BoundaryHighWaterMark" />
  </rdf:Description>
  <rdf:Description rdf:about="http://os.uk/vocabularies/collection/Building-Features">
    <skos:narrower rdf:resource="http://os.uk/vocabularies/ngd/BuildingLine" />
    <skos:narrower rdf:resource="http://os.uk/vocabularies/ngd/BuildingPart" />
  </rdf:Description>
  <rdf:Description rdf:about="https://inspire.ec.europa.eu/metadata-codelist/TopicCategory/structure">
    <skos:narrower rdf:resource="http://os.uk/vocabularies/ngd/BuildingLine" />
    <skos:narrower rdf:resource="http://os.uk/vocabularies/ngd/BuildingPart" />
    <skos:narrower rdf:resource="http://os.uk/vocabularies/ngd/CompoundStructure" />
    <skos:narrower rdf:resource="http://os.uk/vocabularies/ngd/Structure" />
    <skos:narrower rdf:resource="http://os.uk/vocabularies/ngd/StructureLine" />
    <skos:narrower rdf:resource="http://os.uk/vocabularies/ngd/StructurePoint" />
  </rdf:Description>
  <rdf:Description rdf:about="https://inspire.ec.europa.eu/theme/bu">
    <skos:narrower rdf:resource="http://os.uk/vocabularies/ngd/BuildingLine" />
    <skos:narrower rdf:resource="http://os.uk/vocabularies/ngd/BuildingPart" />
    <skos:narrower rdf:resource="http://os.uk/vocabularies/ngd/CompoundStructure" />
    <skos:narrower rdf:resource="http://os.uk/vocabularies/ngd/Structure" />
    <skos:narrower rdf:resource="http://os.uk/vocabularies/ngd/StructureLine" />
    <skos:narrower rdf:resource="http://os.uk/vocabularies/ngd/StructurePoint" />
  </rdf:Description>
  <rdf:Description rdf:about="http://inspire.ec.europa.eu/featureconcept/Building">
    <skos:narrower rdf:resource="http://os.uk/vocabularies/ngd/BuildingLine" />
  </rdf:Description>
  <rdf:Description rdf:about="http://inspire.ec.europa.eu/featureconcept/BuildingPart">
    <skos:narrower rdf:resource="http://os.uk/vocabularies/ngd/BuildingPart" />
  </rdf:Description>
  <rdf:Description rdf:about="http://os.uk/vocabularies/collection/GB-Address">
    <skos:narrower rdf:resource="http://os.uk/vocabularies/ngd/BuiltAddress" />
    <skos:narrower rdf:resource="http://os.uk/vocabularies/ngd/HistoricAddress" />
    <skos:narrower rdf:resource="http://os.uk/vocabularies/ngd/NonAddressableObject" />
    <skos:narrower rdf:resource="http://os.uk/vocabularies/ngd/PreBuildAddress" />
    <skos:narrower rdf:resource="http://os.uk/vocabularies/ngd/StreetAddress" />
  </rdf:Description>
  <rdf:Description rdf:about="http://os.uk/vocabularies/collection/Islands-Address">
    <skos:narrower rdf:resource="http://os.uk/vocabularies/ngd/BuiltAddress" />
    <skos:narrower rdf:resource="http://os.uk/vocabularies/ngd/HistoricAddress" />
    <skos:narrower rdf:resource="http://os.uk/vocabularies/ngd/NonAddressableObject" />
    <skos:narrower rdf:resource="http://os.uk/vocabularies/ngd/PreBuildAddress" />
    <skos:narrower rdf:resource="http://os.uk/vocabularies/ngd/StreetAddress" />
  </rdf:Description>
  <rdf:Description rdf:about="https://inspire.ec.europa.eu/metadata-codelist/TopicCategory/location">
    <skos:narrower rdf:resource="http://os.uk/vocabularies/ngd/BuiltAddress" />
    <skos:narrower rdf:resource="http://os.uk/vocabularies/ngd/HistoricAddress" />
    <skos:narrower rdf:resource="http://os.uk/vocabularies/ngd/NamedArea" />
    <skos:narrower rdf:resource="http://os.uk/vocabularies/ngd/NamedPoint" />
    <skos:narrower rdf:resource="http://os.uk/vocabularies/ngd/NonAddressableObject" />
    <skos:narrower rdf:resource="http://os.uk/vocabularies/ngd/PreBuildAddress" />
    <skos:narrower rdf:resource="http://os.uk/vocabularies/ngd/Site" />
    <skos:narrower rdf:resource="http://os.uk/vocabularies/ngd/StreetAddress" />
  </rdf:Description>
  <rdf:Description rdf:about="https://inspire.ec.europa.eu/theme/ad">
    <skos:narrower rdf:resource="http://os.uk/vocabularies/ngd/BuiltAddress" />
    <skos:narrower rdf:resource="http://os.uk/vocabularies/ngd/HistoricAddress" />
    <skos:narrower rdf:resource="http://os.uk/vocabularies/ngd/NonAddressableObject" />
    <skos:narrower rdf:resource="http://os.uk/vocabularies/ngd/PreBuildAddress" />
    <skos:narrower rdf:resource="http://os.uk/vocabularies/ngd/StreetAddress" />
  </rdf:Description>
  <rdf:Description rdf:about="http://inspire.ec.europa.eu/featureconcept/Address">
    <skos:narrower rdf:resource="http://os.uk/vocabularies/ngd/BuiltAddress" />
    <skos:narrower rdf:resource="http://os.uk/vocabularies/ngd/HistoricAddress" />
    <skos:narrower rdf:resource="http://os.uk/vocabularies/ngd/NonAddressableObject" />
    <skos:narrower rdf:resource="http://os.uk/vocabularies/ngd/PreBuildAddress" />
  </rdf:Description>
  <rdf:Description rdf:about="http://os.uk/vocabularies/collection/Transport-Features">
    <skos:narrower rdf:resource="http://os.uk/vocabularies/ngd/CartographicRailDetail" />
    <skos:narrower rdf:resource="http://os.uk/vocabularies/ngd/CartographicRoadTrackOrPathLine" />
    <skos:narrower rdf:resource="http://os.uk/vocabularies/ngd/RoadLine" />
    <skos:narrower rdf:resource="http://os.uk/vocabularies/ngd/RoadTrackOrPath" />
  </rdf:Description>
  <rdf:Description rdf:about="https://inspire.ec.europa.eu/metadata-codelist/TopicCategory/transportation">
    <skos:narrower rdf:resource="http://os.uk/vocabularies/ngd/CartographicRailDetail" />
    <skos:narrower rdf:resource="http://os.uk/vocabularies/ngd/CartographicRoadTrackOrPathLine" />
    <skos:narrower rdf:resource="http://os.uk/vocabularies/ngd/ConnectingLink" />
    <skos:narrower rdf:resource="http://os.uk/vocabularies/ngd/ConnectingNode" />
    <skos:narrower rdf:resource="http://os.uk/vocabularies/ngd/FerryLink" />
    <skos:narrower rdf:resource="http://os.uk/vocabularies/ngd/FerryNode" />
    <skos:narrower rdf:resource="http://os.uk/vocabularies/ngd/FerryTerminal" />
    <skos:narrower rdf:resource="http://os.uk/vocabularies/ngd/HighwayDedication" />
    <skos:narrower rdf:resource="http://os.uk/vocabularies/ngd/MaintenanceArea" />
    <skos:narrower rdf:resource="http://os.uk/vocabularies/ngd/MaintenanceLine" />
    <skos:narrower rdf:resource="http://os.uk/vocabularies/ngd/MaintenancePoint" />
    <skos:narrower rdf:resource="http://os.uk/vocabularies/ngd/Path" />
    <skos:narrower rdf:resource="http://os.uk/vocabularies/ngd/PathLink" />
    <skos:narrower rdf:resource="http://os.uk/vocabularies/ngd/PathNode" />
    <skos:narrower rdf:resource="http://os.uk/vocabularies/ngd/Rail" />
    <skos:narrower rdf:resource="http://os.uk/vocabularies/ngd/ReinstatementArea" />
    <skos:narrower rdf:resource="http://os.uk/vocabularies/ngd/ReinstatementLine" />
    <skos:narrower rdf:resource="http://os.uk/vocabularies/ngd/ReinstatementPoint" />
    <skos:narrower rdf:resource="http://os.uk/vocabularies/ngd/Restriction" />
    <skos:narrower rdf:resource="http://os.uk/vocabularies/ngd/Road" />
    <skos:narrower rdf:resource="http://os.uk/vocabularies/ngd/RoadJunction" />
    <skos:narrower rdf:resource="http://os.uk/vocabularies/ngd/RoadLine" />
    <skos:narrower rdf:resource="http://os.uk/vocabularies/ngd/RoadLink" />
    <skos:narrower rdf:resource="http://os.uk/vocabularies/ngd/RoadNode" />
    <skos:narrower rdf:resource="http://os.uk/vocabularies/ngd/RoadTrackOrPath" />
    <skos:narrower rdf:resource="http://os.uk/vocabularies/ngd/RoutingHazard" />
    <skos:narrower rdf:resource="http://os.uk/vocabularies/ngd/RoutingStructure" />
    <skos:narrower rdf:resource="http://os.uk/vocabularies/ngd/SiteAccessLocation" />
    <skos:narrower rdf:resource="http://os.uk/vocabularies/ngd/SiteRoutingPoint" />
    <skos:narrower rdf:resource="http://os.uk/vocabularies/ngd/SpecialDesignationArea" />
    <skos:narrower rdf:resource="http://os.uk/vocabularies/ngd/SpecialDesignationLine" />
    <skos:narrower rdf:resource="http://os.uk/vocabularies/ngd/SpecialDesignationPoint" />
    <skos:narrower rdf:resource="http://os.uk/vocabularies/ngd/Street" />
  </rdf:Description>
  <rdf:Description rdf:about="https://inspire.ec.europa.eu/theme/tn">
    <skos:narrower rdf:resource="http://os.uk/vocabularies/ngd/CartographicRailDetail" />
    <skos:narrower rdf:resource="http://os.uk/vocabularies/ngd/CartographicRoadTrackOrPathLine" />
    <skos:narrower rdf:resource="http://os.uk/vocabularies/ngd/ConnectingLink" />
    <skos:narrower rdf:resource="http://os.uk/vocabularies/ngd/ConnectingNode" />
    <skos:narrower rdf:resource="http://os.uk/vocabularies/ngd/FerryLink" />
    <skos:narrower rdf:resource="http://os.uk/vocabularies/ngd/FerryNode" />
    <skos:narrower rdf:resource="http://os.uk/vocabularies/ngd/FerryTerminal" />
    <skos:narrower rdf:resource="http://os.uk/vocabularies/ngd/HighwayDedication" />
    <skos:narrower rdf:resource="http://os.uk/vocabularies/ngd/MaintenanceArea" />
    <skos:narrower rdf:resource="http://os.uk/vocabularies/ngd/MaintenanceLine" />
    <skos:narrower rdf:resource="http://os.uk/vocabularies/ngd/MaintenancePoint" />
    <skos:narrower rdf:resource="http://os.uk/vocabularies/ngd/Path" />
    <skos:narrower rdf:resource="http://os.uk/vocabularies/ngd/PathLink" />
    <skos:narrower rdf:resource="http://os.uk/vocabularies/ngd/PathNode" />
    <skos:narrower rdf:resource="http://os.uk/vocabularies/ngd/Rail" />
    <skos:narrower rdf:resource="http://os.uk/vocabularies/ngd/ReinstatementArea" />
    <skos:narrower rdf:resource="http://os.uk/vocabularies/ngd/ReinstatementLine" />
    <skos:narrower rdf:resource="http://os.uk/vocabularies/ngd/ReinstatementPoint" />
    <skos:narrower rdf:resource="http://os.uk/vocabularies/ngd/Restriction" />
    <skos:narrower rdf:resource="http://os.uk/vocabularies/ngd/Road" />
    <skos:narrower rdf:resource="http://os.uk/vocabularies/ngd/RoadJunction" />
    <skos:narrower rdf:resource="http://os.uk/vocabularies/ngd/RoadLine" />
    <skos:narrower rdf:resource="http://os.uk/vocabularies/ngd/RoadLink" />
    <skos:narrower rdf:resource="http://os.uk/vocabularies/ngd/RoadNode" />
    <skos:narrower rdf:resource="http://os.uk/vocabularies/ngd/RoadTrackOrPath" />
    <skos:narrower rdf:resource="http://os.uk/vocabularies/ngd/RoutingHazard" />
    <skos:narrower rdf:resource="http://os.uk/vocabularies/ngd/RoutingStructure" />
    <skos:narrower rdf:resource="http://os.uk/vocabularies/ngd/SpecialDesignationArea" />
    <skos:narrower rdf:resource="http://os.uk/vocabularies/ngd/SpecialDesignationLine" />
    <skos:narrower rdf:resource="http://os.uk/vocabularies/ngd/SpecialDesignationPoint" />
    <skos:narrower rdf:resource="http://os.uk/vocabularies/ngd/Street" />
  </rdf:Description>
  <rdf:Description rdf:about="http://inspire.ec.europa.eu/featureconcept/Road">
    <skos:narrower rdf:resource="http://os.uk/vocabularies/ngd/CartographicRoadTrackOrPathLine" />
    <skos:narrower rdf:resource="http://os.uk/vocabularies/ngd/Path" />
    <skos:narrower rdf:resource="http://os.uk/vocabularies/ngd/Street" />
  </rdf:Description>
  <rdf:Description rdf:about="http://inspire.ec.europa.eu/featureconcept/AdministrativeUnit">
    <skos:narrower rdf:resource="http://os.uk/vocabularies/ngd/CeremonialCounty" />
    <skos:narrower rdf:resource="http://os.uk/vocabularies/ngd/Country" />
    <skos:narrower rdf:resource="http://os.uk/vocabularies/ngd/DevolvedParliamentConstituency" />
    <skos:narrower rdf:resource="http://os.uk/vocabularies/ngd/DevolvedParliamentElectoralRegion" />
    <skos:narrower rdf:resource="http://os.uk/vocabularies/ngd/ElectoralDivision" />
    <skos:narrower rdf:resource="http://os.uk/vocabularies/ngd/GLAAssemblyConstituency" />
    <skos:narrower rdf:resource="http://os.uk/vocabularies/ngd/HistoricCounty" />
    <skos:narrower rdf:resource="http://os.uk/vocabularies/ngd/HistoricEuropeanRegion" />
    <skos:narrower rdf:resource="http://os.uk/vocabularies/ngd/LowerTierLocalAuthority" />
    <skos:narrower rdf:resource="http://os.uk/vocabularies/ngd/ParishOrCommunity" />
    <skos:narrower rdf:resource="http://os.uk/vocabularies/ngd/PollingDistrict" />
    <skos:narrower rdf:resource="http://os.uk/vocabularies/ngd/Region" />
    <skos:narrower rdf:resource="http://os.uk/vocabularies/ngd/RegionalAuthority" />
    <skos:narrower rdf:resource="http://os.uk/vocabularies/ngd/UpperTierLocalAuthority" />
    <skos:narrower rdf:resource="http://os.uk/vocabularies/ngd/Ward" />
    <skos:narrower rdf:resource="http://os.uk/vocabularies/ngd/WestminsterConstituency" />
  </rdf:Description>
  <rdf:Description rdf:about="http://os.uk/vocabularies/collection/Structure-Features">
    <skos:narrower rdf:resource="http://os.uk/vocabularies/ngd/CompoundStructure" />
    <skos:narrower rdf:resource="http://os.uk/vocabularies/ngd/Structure" />
    <skos:narrower rdf:resource="http://os.uk/vocabularies/ngd/StructureLine" />
    <skos:narrower rdf:resource="http://os.uk/vocabularies/ngd/StructurePoint" />
  </rdf:Description>
  <rdf:Description rdf:about="http://os.uk/vocabularies/collection/Transport-Network">
    <skos:narrower rdf:resource="http://os.uk/vocabularies/ngd/ConnectingLink" />
    <skos:narrower rdf:resource="http://os.uk/vocabularies/ngd/ConnectingNode" />
    <skos:narrower rdf:resource="http://os.uk/vocabularies/ngd/FerryLink" />
    <skos:narrower rdf:resource="http://os.uk/vocabularies/ngd/FerryNode" />
    <skos:narrower rdf:resource="http://os.uk/vocabularies/ngd/FerryTerminal" />
    <skos:narrower rdf:resource="http://os.uk/vocabularies/ngd/Path" />
    <skos:narrower rdf:resource="http://os.uk/vocabularies/ngd/PathLink" />
    <skos:narrower rdf:resource="http://os.uk/vocabularies/ngd/PathNode" />
    <skos:narrower rdf:resource="http://os.uk/vocabularies/ngd/Rail" />
    <skos:narrower rdf:resource="http://os.uk/vocabularies/ngd/Road" />
    <skos:narrower rdf:resource="http://os.uk/vocabularies/ngd/RoadJunction" />
    <skos:narrower rdf:resource="http://os.uk/vocabularies/ngd/RoadLink" />
    <skos:narrower rdf:resource="http://os.uk/vocabularies/ngd/RoadNode" />
    <skos:narrower rdf:resource="http://os.uk/vocabularies/ngd/Street" />
  </rdf:Description>
  <rdf:Description rdf:about="http://inspire.ec.europa.eu/featureconcept/RoadLink">
    <skos:narrower rdf:resource="http://os.uk/vocabularies/ngd/ConnectingLink" />
    <skos:narrower rdf:resource="http://os.uk/vocabularies/ngd/PathLink" />
  </rdf:Description>
  <rdf:Description rdf:about="http://inspire.ec.europa.eu/featureconcept/RoadNode">
    <skos:narrower rdf:resource="http://os.uk/vocabularies/ngd/ConnectingNode" />
    <skos:narrower rdf:resource="http://os.uk/vocabularies/ngd/PathNode" />
    <skos:narrower rdf:resource="http://os.uk/vocabularies/ngd/RoadJunction" />
  </rdf:Description>
  <rdf:Description rdf:about="http://inspire.ec.europa.eu/featureconcept/PortNode">
    <skos:narrower rdf:resource="http://os.uk/vocabularies/ngd/FerryNode" />
    <skos:narrower rdf:resource="http://os.uk/vocabularies/ngd/FerryTerminal" />
  </rdf:Description>
  <rdf:Description rdf:about="http://os.uk/vocabularies/collection/RAMI">
    <skos:narrower rdf:resource="http://os.uk/vocabularies/ngd/HighwayDedication" />
    <skos:narrower rdf:resource="http://os.uk/vocabularies/ngd/MaintenanceArea" />
    <skos:narrower rdf:resource="http://os.uk/vocabularies/ngd/MaintenanceLine" />
    <skos:narrower rdf:resource="http://os.uk/vocabularies/ngd/MaintenancePoint" />
    <skos:narrower rdf:resource="http://os.uk/vocabularies/ngd/ReinstatementArea" />
    <skos:narrower rdf:resource="http://os.uk/vocabularies/ngd/ReinstatementLine" />
    <skos:narrower rdf:resource="http://os.uk/vocabularies/ngd/ReinstatementPoint" />
    <skos:narrower rdf:resource="http://os.uk/vocabularies/ngd/Restriction" />
    <skos:narrower rdf:resource="http://os.uk/vocabularies/ngd/RoutingHazard" />
    <skos:narrower rdf:resource="http://os.uk/vocabularies/ngd/RoutingStructure" />
    <skos:narrower rdf:resource="http://os.uk/vocabularies/ngd/SpecialDesignationArea" />
    <skos:narrower rdf:resource="http://os.uk/vocabularies/ngd/SpecialDesignationLine" />
    <skos:narrower rdf:resource="http://os.uk/vocabularies/ngd/SpecialDesignationPoint" />
  </rdf:Description>
  <rdf:Description rdf:about="http://inspire.ec.europa.eu/featureconcept/RestrictionForVehicles">
    <skos:narrower rdf:resource="http://os.uk/vocabularies/ngd/HighwayDedication" />
  </rdf:Description>
  <rdf:Description rdf:about="http://os.uk/vocabularies/collection/Water-Features">
    <skos:narrower rdf:resource="http://os.uk/vocabularies/ngd/InterTidalLine" />
    <skos:narrower rdf:resource="http://os.uk/vocabularies/ngd/TidalBoundary" />
    <skos:narrower rdf:resource="http://os.uk/vocabularies/ngd/Water" />
    <skos:narrower rdf:resource="http://os.uk/vocabularies/ngd/WaterPoint" />
  </rdf:Description>
  <rdf:Description rdf:about="https://inspire.ec.europa.eu/metadata-codelist/TopicCategory/inlandWaters">
    <skos:narrower rdf:resource="http://os.uk/vocabularies/ngd/InterTidalLine" />
    <skos:narrower rdf:resource="http://os.uk/vocabularies/ngd/Water" />
    <skos:narrower rdf:resource="http://os.uk/vocabularies/ngd/WaterLink" />
    <skos:narrower rdf:resource="http://os.uk/vocabularies/ngd/WaterLinkSet" />
    <skos:narrower rdf:resource="http://os.uk/vocabularies/ngd/WaterNode" />
    <skos:narrower rdf:resource="http://os.uk/vocabularies/ngd/WaterPoint" />
  </rdf:Description>
  <rdf:Description rdf:about="https://inspire.ec.europa.eu/theme/hy">
    <skos:narrower rdf:resource="http://os.uk/vocabularies/ngd/InterTidalLine" />
    <skos:narrower rdf:resource="http://os.uk/vocabularies/ngd/TidalBoundary" />
    <skos:narrower rdf:resource="http://os.uk/vocabularies/ngd/Water" />
    <skos:narrower rdf:resource="http://os.uk/vocabularies/ngd/WaterLink" />
    <skos:narrower rdf:resource="http://os.uk/vocabularies/ngd/WaterLinkSet" />
    <skos:narrower rdf:resource="http://os.uk/vocabularies/ngd/WaterNode" />
    <skos:narrower rdf:resource="http://os.uk/vocabularies/ngd/WaterPoint" />
  </rdf:Description>
  <rdf:Description rdf:about="https://inspire.ec.europa.eu/featureconcept/Watercourse">
    <skos:narrower rdf:resource="http://os.uk/vocabularies/ngd/InterTidalLine" />
  </rdf:Description>
  <rdf:Description rdf:about="http://os.uk/vocabularies/collection/Land-Features">
    <skos:narrower rdf:resource="http://os.uk/vocabularies/ngd/Land" />
    <skos:narrower rdf:resource="http://os.uk/vocabularies/ngd/Landform" />
    <skos:narrower rdf:resource="http://os.uk/vocabularies/ngd/LandformLine" />
    <skos:narrower rdf:resource="http://os.uk/vocabularies/ngd/LandformPoint" />
  </rdf:Description>
  <rdf:Description rdf:about="https://inspire.ec.europa.eu/metadata-codelist/TopicCategory/imageryBaseMapsEarthCover">
    <skos:narrower rdf:resource="http://os.uk/vocabularies/ngd/Land" />
  </rdf:Description>
  <rdf:Description rdf:about="https://inspire.ec.europa.eu/theme/lc">
    <skos:narrower rdf:resource="http://os.uk/vocabularies/ngd/Land" />
  </rdf:Description>
  <rdf:Description rdf:about="http://inspire.ec.europa.eu/featureconcept/LandCoverUnit">
    <skos:narrower rdf:resource="http://os.uk/vocabularies/ngd/Land" />
  </rdf:Description>
  <rdf:Description rdf:about="https://inspire.ec.europa.eu/metadata-codelist/TopicCategory/environment">
    <skos:narrower rdf:resource="http://os.uk/vocabularies/ngd/Landform" />
    <skos:narrower rdf:resource="http://os.uk/vocabularies/ngd/LandformLine" />
    <skos:narrower rdf:resource="http://os.uk/vocabularies/ngd/LandformPoint" />
  </rdf:Description>
  <rdf:Description rdf:about="http://inspire.ec.europa.eu/featureconcept/MaintenanceAuthority">
    <skos:narrower rdf:resource="http://os.uk/vocabularies/ngd/MaintenanceLine" />
    <skos:narrower rdf:resource="http://os.uk/vocabularies/ngd/MaintenancePoint" />
  </rdf:Description>
  <rdf:Description rdf:about="http://os.uk/vocabularies/collection/Named-Features">
    <skos:narrower rdf:resource="http://os.uk/vocabularies/ngd/NamedArea" />
    <skos:narrower rdf:resource="http://os.uk/vocabularies/ngd/NamedPoint" />
  </rdf:Description>
  <rdf:Description rdf:about="https://inspire.ec.europa.eu/theme/gn">
    <skos:narrower rdf:resource="http://os.uk/vocabularies/ngd/NamedArea" />
    <skos:narrower rdf:resource="http://os.uk/vocabularies/ngd/NamedPoint" />
  </rdf:Description>
  <rdf:Description rdf:about="http://inspire.ec.europa.eu/featureconcept/NamedPlace">
    <skos:narrower rdf:resource="http://os.uk/vocabularies/ngd/NamedArea" />
    <skos:narrower rdf:resource="http://os.uk/vocabularies/ngd/NamedPoint" />
  </rdf:Description>
  <rdf:Description rdf:about="http://inspire.ec.europa.eu/featureconcept/RailwayArea">
    <skos:narrower rdf:resource="http://os.uk/vocabularies/ngd/Rail" />
  </rdf:Description>
  <rdf:Description rdf:about="http://inspire.ec.europa.eu/featureconcept/RoadLinkSequence">
    <skos:narrower rdf:resource="http://os.uk/vocabularies/ngd/RoadLine" />
    <skos:narrower rdf:resource="http://os.uk/vocabularies/ngd/RoadTrackOrPath" />
  </rdf:Description>
  <rdf:Description rdf:about="http://os.uk/vocabularies/collection/Land-Use-Features">
    <skos:narrower rdf:resource="http://os.uk/vocabularies/ngd/Site" />
    <skos:narrower rdf:resource="http://os.uk/vocabularies/ngd/SiteAccessLocation" />
    <skos:narrower rdf:resource="http://os.uk/vocabularies/ngd/SiteRoutingPoint" />
  </rdf:Description>
  <rdf:Description rdf:about="http://inspire.ec.europa.eu/featureconcept/ThoroughfareName">
    <skos:narrower rdf:resource="http://os.uk/vocabularies/ngd/StreetAddress" />
  </rdf:Description>
  <rdf:Description rdf:about="https://inspire.ec.europa.eu/metadata-codelist/TopicCategory/oceans">
    <skos:narrower rdf:resource="http://os.uk/vocabularies/ngd/TidalBoundary" />
  </rdf:Description>
  <rdf:Description rdf:about="http://inspire.ec.europa.eu/featureconcept/LandWaterBoundary">
    <skos:narrower rdf:resource="http://os.uk/vocabularies/ngd/TidalBoundary" />
  </rdf:Description>
  <rdf:Description rdf:about="http://inspire.ec.europa.eu/featureconcept/StandingWater">
    <skos:narrower rdf:resource="http://os.uk/vocabularies/ngd/Water" />
  </rdf:Description>
  <rdf:Description rdf:about="http://os.uk/vocabularies/collection/Water-Network">
    <skos:narrower rdf:resource="http://os.uk/vocabularies/ngd/WaterLink" />
    <skos:narrower rdf:resource="http://os.uk/vocabularies/ngd/WaterLinkSet" />
    <skos:narrower rdf:resource="http://os.uk/vocabularies/ngd/WaterNode" />
  </rdf:Description>
  <rdf:Description rdf:about="http://inspire.ec.europa.eu/featureconcept/Watercourse">
    <skos:narrower rdf:resource="http://os.uk/vocabularies/ngd/WaterLinkSet" />
  </rdf:Description>
  <rdf:Description rdf:about="http://os.uk/vocabularies/themes">
    <rdf:type rdf:resource="http://www.w3.org/2004/02/skos/core#ConceptScheme" />
    <dct:title xml:lang="en">Ordnance Survey NGD themes</dct:title>
    <dct:description xml:lang="en">Pre-release trial SKOS version of evolving NGD vocab, 2022-02-15 extract from NGD_Metadata_And_Definitions_MASTER</dct:description>
    <skos:hasTopConcept rdf:resource="http://os.uk/vocabularies/ngd" />
    <skos:hasTopConcept rdf:resource="http://os.uk/vocabularies/theme/add" />
    <skos:hasTopConcept rdf:resource="http://os.uk/vocabularies/theme/asu" />
    <skos:hasTopConcept rdf:resource="http://os.uk/vocabularies/theme/bld" />
    <skos:hasTopConcept rdf:resource="http://os.uk/vocabularies/theme/trn" />
    <skos:hasTopConcept rdf:resource="http://os.uk/vocabularies/theme/str" />
    <skos:hasTopConcept rdf:resource="http://os.uk/vocabularies/theme/wtr" />
    <skos:hasTopConcept rdf:resource="http://os.uk/vocabularies/theme/gnm" />
    <skos:hasTopConcept rdf:resource="http://os.uk/vocabularies/theme/lnd" />
    <skos:hasTopConcept rdf:resource="http://os.uk/vocabularies/theme/lus" />
  </rdf:Description>
  <rdf:Description rdf:about="http://os.uk/vocabularies/ngd">
    <rdf:type rdf:resource="http://www.w3.org/2004/02/skos/core#Concept" />
    <skos:prefLabel xml:lang="en">National Geographic Database</skos:prefLabel>
    <skos:definition xml:lang="en">The National Geographic Database (NGD) contains the authoritative data that describes the geography of Great Britain</skos:definition>
    <skos:inScheme rdf:resource="http://os.uk/vocabularies/themes" />
    <skos:topConceptOf rdf:resource="http://os.uk/vocabularies/themes" />
  </rdf:Description>
  <rdf:Description rdf:about="http://os.uk/vocabularies/theme/add">
    <rdf:type rdf:resource="http://www.w3.org/2004/02/skos/core#Concept" />
    <skos:prefLabel xml:lang="en">Address</skos:prefLabel>
    <skos:definition xml:lang="en">The address theme contains point locations for addresses within GB and beyond</skos:definition>
    <skos:narrower rdf:resource="http://os.uk/vocabularies/collection/GB-Address" />
    <skos:narrower rdf:resource="http://os.uk/vocabularies/collection/Islands-Address" />
    <skos:inScheme rdf:resource="http://os.uk/vocabularies/themes" />
    <skos:topConceptOf rdf:resource="http://os.uk/vocabularies/themes" />
  </rdf:Description>
  <rdf:Description rdf:about="http://os.uk/vocabularies/theme/asu">
    <rdf:type rdf:resource="http://www.w3.org/2004/02/skos/core#Concept" />
    <skos:prefLabel xml:lang="en">Administrative And Statistical Units</skos:prefLabel>
    <skos:definition xml:lang="en">The boundary theme contains data which provides a representation of the hierarchy of administrative and electoral boundaries and their names for England, Scotland and Wales</skos:definition>
    <skos:narrower rdf:resource="http://os.uk/vocabularies/collection/Boundaries" />
    <skos:inScheme rdf:resource="http://os.uk/vocabularies/themes" />
    <skos:topConceptOf rdf:resource="http://os.uk/vocabularies/themes" />
  </rdf:Description>
  <rdf:Description rdf:about="http://os.uk/vocabularies/theme/bld">
    <rdf:type rdf:resource="http://www.w3.org/2004/02/skos/core#Concept" />
    <skos:prefLabel xml:lang="en">Buildings</skos:prefLabel>
    <skos:definition xml:lang="en">The building theme contains buildings which meet the defintion of a permanent roofed construction, usually with walls.</skos:definition>
    <skos:narrower rdf:resource="http://os.uk/vocabularies/collection/Building-Features" />
    <skos:inScheme rdf:resource="http://os.uk/vocabularies/themes" />
    <skos:topConceptOf rdf:resource="http://os.uk/vocabularies/themes" />
  </rdf:Description>
  <rdf:Description rdf:about="http://os.uk/vocabularies/theme/trn">
    <rdf:type rdf:resource="http://www.w3.org/2004/02/skos/core#Concept" />
    <skos:prefLabel xml:lang="en">Transport</skos:prefLabel>
    <skos:definition xml:lang="en">The transport theme contains both the geographical representation and routing network for Great Britains highway information.</skos:definition>
    <skos:narrower rdf:resource="http://os.uk/vocabularies/collection/RAMI" />
    <skos:narrower rdf:resource="http://os.uk/vocabularies/collection/Transport-Features" />
    <skos:narrower rdf:resource="http://os.uk/vocabularies/collection/Transport-Network" />
    <skos:inScheme rdf:resource="http://os.uk/vocabularies/themes" />
    <skos:topConceptOf rdf:resource="http://os.uk/vocabularies/themes" />
  </rdf:Description>
  <rdf:Description rdf:about="http://os.uk/vocabularies/theme/str">
    <rdf:type rdf:resource="http://www.w3.org/2004/02/skos/core#Concept" />
    <skos:prefLabel xml:lang="en">Structures</skos:prefLabel>
    <skos:definition xml:lang="en">The structures theme contains features which are of manmade construction but not a building.</skos:definition>
    <skos:narrower rdf:resource="http://os.uk/vocabularies/collection/Structure-Features" />
    <skos:inScheme rdf:resource="http://os.uk/vocabularies/themes" />
    <skos:topConceptOf rdf:resource="http://os.uk/vocabularies/themes" />
  </rdf:Description>
  <rdf:Description rdf:about="http://os.uk/vocabularies/theme/wtr">
    <rdf:type rdf:resource="http://www.w3.org/2004/02/skos/core#Concept" />
    <skos:prefLabel xml:lang="en">Water</skos:prefLabel>
    <skos:definition xml:lang="en">The water theme contains features which are defined as features that contain, delimit, or relate to real-world objects containing water; as well as a three-dimensional structured link and node network of watercourses for Great Britain.</skos:definition>
    <skos:narrower rdf:resource="http://os.uk/vocabularies/collection/Water-Features" />
    <skos:narrower rdf:resource="http://os.uk/vocabularies/collection/Water-Network" />
    <skos:inScheme rdf:resource="http://os.uk/vocabularies/themes" />
    <skos:topConceptOf rdf:resource="http://os.uk/vocabularies/themes" />
  </rdf:Description>
  <rdf:Description rdf:about="http://os.uk/vocabularies/theme/gnm">
    <rdf:type rdf:resource="http://www.w3.org/2004/02/skos/core#Concept" />
    <skos:prefLabel xml:lang="en">Geographical Names</skos:prefLabel>
    <skos:definition xml:lang="en">The Geographical Names theme contains named water, land and settlement features.</skos:definition>
    <skos:narrower rdf:resource="http://os.uk/vocabularies/collection/Named-Features" />
    <skos:inScheme rdf:resource="http://os.uk/vocabularies/themes" />
    <skos:topConceptOf rdf:resource="http://os.uk/vocabularies/themes" />
  </rdf:Description>
  <rdf:Description rdf:about="http://os.uk/vocabularies/theme/lnd">
    <rdf:type rdf:resource="http://www.w3.org/2004/02/skos/core#Concept" />
    <skos:prefLabel xml:lang="en">Land</skos:prefLabel>
    <skos:narrower rdf:resource="http://os.uk/vocabularies/collection/Land-Features" />
    <skos:inScheme rdf:resource="http://os.uk/vocabularies/themes" />
    <skos:topConceptOf rdf:resource="http://os.uk/vocabularies/themes" />
  </rdf:Description>
  <rdf:Description rdf:about="http://os.uk/vocabularies/theme/lus">
    <rdf:type rdf:resource="http://www.w3.org/2004/02/skos/core#Concept" />
    <skos:prefLabel xml:lang="en">Land Use</skos:prefLabel>
    <skos:definition xml:lang="en">The land use theme provides a polygon extent of a function or activity as well as the entrance point and a routing point location.</skos:definition>
    <skos:narrower rdf:resource="http://os.uk/vocabularies/collection/Land-Use-Features" />
    <skos:inScheme rdf:resource="http://os.uk/vocabularies/themes" />
    <skos:topConceptOf rdf:resource="http://os.uk/vocabularies/themes" />
  </rdf:Description>
  <rdf:Description rdf:about="http://os.uk/vocabularies/collection/Boundaries">
    <rdf:type rdf:resource="http://www.w3.org/2004/02/skos/core#Concept" />
    <skos:prefLabel xml:lang="en">Boundaries</skos:prefLabel>
    <skos:definition xml:lang="en">Boundary features which provide a representation of the hierarchy of administrative and electoral boundaries and their names for England, Scotland and Wales</skos:definition>
    <skos:broader rdf:resource="http://os.uk/vocabularies/theme/asu" />
    <skos:inScheme rdf:resource="http://os.uk/vocabularies/themes" />
  </rdf:Description>
  <rdf:Description rdf:about="http://os.uk/vocabularies/collection/Building-Features">
    <rdf:type rdf:resource="http://www.w3.org/2004/02/skos/core#Concept" />
    <skos:prefLabel xml:lang="en">Building-Features</skos:prefLabel>
    <skos:definition xml:lang="en">Building features which meet the defintion of a permanent roofed construction, usually with walls.</skos:definition>
    <skos:broader rdf:resource="http://os.uk/vocabularies/theme/bld" />
    <skos:inScheme rdf:resource="http://os.uk/vocabularies/themes" />
  </rdf:Description>
  <rdf:Description rdf:about="http://os.uk/vocabularies/collection/GB-Address">
    <rdf:type rdf:resource="http://www.w3.org/2004/02/skos/core#Concept" />
    <skos:prefLabel xml:lang="en">GB-Address</skos:prefLabel>
    <skos:definition xml:lang="en">Address features which fall within Great Britain (England, Wales and Scotland)</skos:definition>
    <skos:broader rdf:resource="http://os.uk/vocabularies/theme/add" />
    <skos:inScheme rdf:resource="http://os.uk/vocabularies/themes" />
  </rdf:Description>
  <rdf:Description rdf:about="http://os.uk/vocabularies/collection/Islands-Address">
    <rdf:type rdf:resource="http://www.w3.org/2004/02/skos/core#Concept" />
    <skos:prefLabel xml:lang="en">Islands-Address</skos:prefLabel>
    <skos:definition xml:lang="en">Address features which fall within either Northern Ireland, Isle of Man or the Channel Islands</skos:definition>
    <skos:broader rdf:resource="http://os.uk/vocabularies/theme/add" />
    <skos:inScheme rdf:resource="http://os.uk/vocabularies/themes" />
  </rdf:Description>
  <rdf:Description rdf:about="http://os.uk/vocabularies/collection/Land-Features">
    <rdf:type rdf:resource="http://www.w3.org/2004/02/skos/core#Concept" />
    <skos:prefLabel xml:lang="en">Land-Features</skos:prefLabel>
    <skos:definition xml:lang="en">Land use features provided as a polygon and represents the extent of a function or activity</skos:definition>
    <skos:broader rdf:resource="http://os.uk/vocabularies/theme/lnd" />
    <skos:inScheme rdf:resource="http://os.uk/vocabularies/themes" />
  </rdf:Description>
  <rdf:Description rdf:about="http://os.uk/vocabularies/collection/Land-Use-Features">
    <rdf:type rdf:resource="http://www.w3.org/2004/02/skos/core#Concept" />
    <skos:prefLabel xml:lang="en">Land-Use-Features</skos:prefLabel>
    <skos:definition xml:lang="en">Land use features provided as a polygon representing the extent of a function or activity, connected to the transport network</skos:definition>
    <skos:broader rdf:resource="http://os.uk/vocabularies/theme/lus" />
    <skos:inScheme rdf:resource="http://os.uk/vocabularies/themes" />
  </rdf:Description>
  <rdf:Description rdf:about="http://os.uk/vocabularies/collection/Named-Features">
    <rdf:type rdf:resource="http://www.w3.org/2004/02/skos/core#Concept" />
    <skos:prefLabel xml:lang="en">Named-Features</skos:prefLabel>
    <skos:definition xml:lang="en">Geographical names for water, land and settlement locations.</skos:definition>
    <skos:broader rdf:resource="http://os.uk/vocabularies/theme/gnm" />
    <skos:inScheme rdf:resource="http://os.uk/vocabularies/themes" />
  </rdf:Description>
  <rdf:Description rdf:about="http://os.uk/vocabularies/collection/RAMI">
    <rdf:type rdf:resource="http://www.w3.org/2004/02/skos/core#Concept" />
    <skos:prefLabel xml:lang="en">RAMI</skos:prefLabel>
    <skos:broader rdf:resource="http://os.uk/vocabularies/theme/trn" />
    <skos:inScheme rdf:resource="http://os.uk/vocabularies/themes" />
  </rdf:Description>
  <rdf:Description rdf:about="http://os.uk/vocabularies/collection/Structure-Features">
    <rdf:type rdf:resource="http://www.w3.org/2004/02/skos/core#Concept" />
    <skos:prefLabel xml:lang="en">Structure-Features</skos:prefLabel>
    <skos:definition xml:lang="en">Structure features which are of manmade construction but not a building.</skos:definition>
    <skos:broader rdf:resource="http://os.uk/vocabularies/theme/str" />
    <skos:inScheme rdf:resource="http://os.uk/vocabularies/themes" />
  </rdf:Description>
  <rdf:Description rdf:about="http://os.uk/vocabularies/collection/Transport-Features">
    <rdf:type rdf:resource="http://www.w3.org/2004/02/skos/core#Concept" />
    <skos:prefLabel xml:lang="en">Transport-Features</skos:prefLabel>
    <skos:broader rdf:resource="http://os.uk/vocabularies/theme/trn" />
    <skos:inScheme rdf:resource="http://os.uk/vocabularies/themes" />
  </rdf:Description>
  <rdf:Description rdf:about="http://os.uk/vocabularies/collection/Transport-Network">
    <rdf:type rdf:resource="http://www.w3.org/2004/02/skos/core#Concept" />
    <skos:prefLabel xml:lang="en">Transport-Network</skos:prefLabel>
    <skos:broader rdf:resource="http://os.uk/vocabularies/theme/trn" />
    <skos:inScheme rdf:resource="http://os.uk/vocabularies/themes" />
  </rdf:Description>
  <rdf:Description rdf:about="http://os.uk/vocabularies/collection/Water-Features">
    <rdf:type rdf:resource="http://www.w3.org/2004/02/skos/core#Concept" />
    <skos:prefLabel xml:lang="en">Water-Features</skos:prefLabel>
    <skos:definition xml:lang="en">Water features that contain, delimit, or relate to real-world objects containing water</skos:definition>
    <skos:broader rdf:resource="http://os.uk/vocabularies/theme/wtr" />
    <skos:inScheme rdf:resource="http://os.uk/vocabularies/themes" />
  </rdf:Description>
  <rdf:Description rdf:about="http://os.uk/vocabularies/collection/Water-Network">
    <rdf:type rdf:resource="http://www.w3.org/2004/02/skos/core#Concept" />
    <skos:prefLabel xml:lang="en">Water-Network</skos:prefLabel>
    <skos:definition xml:lang="en">A three-dimensional structured link and node network of watercourses for Great Britain.</skos:definition>
    <skos:broader rdf:resource="http://os.uk/vocabularies/theme/wtr" />
    <skos:inScheme rdf:resource="http://os.uk/vocabularies/themes" />
  </rdf:Description>
</rdf:RDF>

